Proved preliminary version of trans_m_iso_pre_post

doc/coq/simple/Equiv.v
@@ -827,44 +827,6 @@ Proof.
   repeat des_goal; clarify; eauto.
 Qed.
 
-Lemma ϕ_spec_app `{Eq TT} `{Eq aTT} `{TotalOrder T} `{Eq aT}
-  (α' : TT -> aTT) (α : T -> aT) (φ : aTT -> aT) (φ' : aT -> aTT) :
-  forall (ϕ1 ϕ2 : list (TT * T)) (t : T)
-    (SPECϕ : ϕ_spec α' α φ φ' (ϕ1 ++ ϕ2) t),
-  ϕ_spec α' α φ φ' ϕ1 t /\ ϕ_spec α' α φ φ' ϕ2 t.
-Proof.
-  induction ϕ1; ii; ss.
-  assert (ϕ_spec α' α φ φ' (ϕ1 ++ ϕ2) t).
-  {
-    ii. exploit (SPECϕ t'' t'); eauto.
-    ss. rewrite in_app_iff in *. des; eauto.
-    ii. des. ss. repeat des_hyp; clarify;
-    first [rewrite t_refl in *; clarify |
-      rewrite eqb_eq in *; clarify].
-    repeat split; eauto.
-    apply in_read_fst in IN as READ. des.
-    apply read_fst_in in READ as IN'.
-    exploit (SPECϕ t0 t''); ss; eauto.
-    rewrite t_refl. ii; des; clarify.
-    apply in_read_snd in IN as READ. des.
-    apply read_snd_in in READ as IN'.
-    exploit (SPECϕ t'' t1); ss; eauto.
-    rewrite t_refl. ii; des; clarify.
-  }
-  exploit IHϕ1; eauto.
-  ii. des. split; eauto.
-  ii. ss.
-  exploit (SPECϕ t'' t'). ss. rewrite in_app_iff.
-  des; eauto. ii. des; clarify.
-  - repeat rewrite t_refl. eauto.
-  - exploit (x0 t'' t'). eauto.
-    ii. des; clarify.
-    ss.
-    rewrite read_fst_top in *.
-    rewrite read_snd_top in *.
-    repeat des_hyp; clarify.
-Qed.
-
 Fixpoint pmap_fst `{Eq T} `{Eq TT} (ϕ: list (T * TT)) (p : path T) :=
   match p with
   | Pnil => Some Pnil
@@ -1618,13 +1580,26 @@ Lemma remove_t_dec `{Eq T} :
   forall (m : memory T) t,
   (List.length (remove_t m t)) <= (List.length m).
 Proof.
-  induction m; intros; simpl; eauto.
+  induction m; intros; simpl; eauto;
   repeat des_goal; repeat des_hyp; clarify;
   try rewrite eqb_eq in *; subst;
   match goal with
   | |- context [remove_t _ ?t] =>
     specialize (IHm t); nia
   end.
+Qed.
+
+Lemma remove_t_strict_dec `{Eq T} :
+  forall (m : memory T) t (READ : None <> read m t),
+  (List.length (remove_t m t)) < (List.length m).
+Proof.
+  induction m; intros; simpl; eauto; clarify;
+  repeat des_goal; repeat des_hyp; clarify;
+  try rewrite eqb_eq in *; subst.
+  pose proof (remove_t_dec m t0). nia.
+  ss. rewrite eqb_comm in GDES0.
+  revert READ. rw. ii. exploit IHm; eauto.
+  nia.
 Qed.
 
 Lemma remove_t_read `{Eq T} :
@@ -1864,7 +1839,7 @@ Definition trans_m_step_post `{Eq TT} `{Eq aTT} `{TotalOrder T} `{Eq aT}
     forall t' (IN : None <> read_fst ϕ t'),
       None = read m' t'
   | Changed t' (Closure x' e' C') t (Closure x e C) ϕ_af tϕ_af =>
-    None <> read_fst ϕ t' /\ x' = x /\ e' = e /\
+    Some t = read_fst ϕ t' /\ x' = x /\ e' = e /\
     Some (Closure x' e' C') = read m' t' /\
     In (Closure x e (trans_C α C)) (aread m (α t)) /\
     ϕ_spec α' α φ φ' ϕ_af tϕ_af /\
@@ -1920,10 +1895,6 @@ Proof.
       ii; des; eauto].
 Qed.
 
-Definition reachϕ `{Eq T} `{Eq TT} (ϕ : list (T * TT)) (m : memory T) t :=
-  None <> read_fst ϕ t \/
-  exists t', None <> read_fst ϕ t' /\ reachable (Ptr t') m t.
-
 Lemma trans_m_step_pre_post `{Eq TT} `{Eq aTT} `{TotalOrder T} `{Eq aT}
   (α' : TT -> aTT) (inv_α : (T * aT) -> T) (α : T -> aT) 
   (SPECα : inv_α_spec α inv_α) φ φ' :
@@ -1950,7 +1921,7 @@ Proof.
     intros POST. unfold trans_iso_C_post in POST.
     repeat des_hyp; clarify.
     rewrite t_refl. des; clarify.
-    repeat (split; eauto). rw. ii. clarify.
+    repeat (split; eauto).
     exploit (SPECϕ t' t).
     symmetry in CASE. apply read_fst_in in CASE. eauto.
     ii. des. rw. eauto.
@@ -1969,7 +1940,7 @@ Proof.
     repeat des_hyp; des; clarify.
     assert (eqb t' t = false).
     {
-      rewrite eqb_neq. ii. clarify. eauto.
+      rewrite eqb_neq. ii. clarify. rewrite CASE in *. clarify.
     }
     rw. repeat (split; eauto).
 Qed.
@@ -2060,1903 +2031,434 @@ Proof.
     exists (Closure x e C). eauto.
 Qed.
 
-(*
-
-
-Definition eq_edge `{Eq T} (e e' : edge T) :=
-  match e, e' with
-  | Ex nC x ntx, Ex nC' x' ntx' =>
-    eqb nC nC' && eqb x x' && eqb ntx ntx'
-  | EM nC M nCM, EM nC' M' nCM' =>
-    eqb nC nC' && eqb M M' && eqb nCM nCM'
-  | Ev nt v nCv, Ev nt' v' nCv' =>
-    eqb nt nt' && eqb v v' && eqb nCv nCv'
-  | _, _ => false
-  end.
-
-Lemma eq_edge_eq `{Eq T} :
-  forall e e', eq_edge e e' = true <-> e = e'.
-Proof.
-  ii. unfold eq_edge.
-  repeat des_goal; repeat des_hyp;
-  try rewrite eqb_ID_eq in *; 
-  try rewrite eqb_ID_neq in *;
-  try rewrite eq_node_eq in *;
-  try rewrite eq_node_neq in *;
-  try rewrite eq_val_eq in *;
-  try rewrite eq_val_neq in *;
-  split; ii; clarify.
-Qed.
-
-#[export] Instance EqEdge `{Eq T} : Eq (edge T) :=
-  { eqb := eq_edge; eqb_eq := eq_edge_eq; }.
-
-Lemma eq_edge_neq `{Eq T} :
-  forall e e', eq_edge e e' = false <-> e <> e'.
-Proof.
-  assert (eq_edge = eqb) as RR. eauto.
-  rewrite RR. exact eqb_neq.
-Qed.
-
-Definition valid_edge `{Eq T} (m : memory T) (e : edge T) :=
-  match e with
-  | Ex (Ctx C) x (Ptr tx) =>
-    match addr_x C x with
-    | Some t => t = tx
+Definition equiv_fst_ϕ_m `{Eq T} `{Eq TT} (ϕ : list (T * TT)) m m' :=
+  forall t p x e C
+  (READ : Some (Closure x e C) = read m t)
+  (VALp : valid_path (Ctx C) [] p),
+  match read_fst ϕ t with
+  | Some t' =>
+    match pmap_fst ϕ p with
+    | Some p' =>
+      exists C', Some (Closure x e C') = read m' t' /\
+        valid_path (Ctx C') [] p'
     | None => False
-    end
-  | EM (Ctx C) M (Ctx CM) =>
-    match ctx_M C M with
-    | Some C => C = CM
+    end 
+  | None => False
+  end.
+
+Definition equiv_snd_ϕ_m `{Eq T} `{Eq TT} (ϕ : list (T * TT)) m m' :=
+  forall t p x e C
+  (READ : Some (Closure x e C) = read m t)
+  (VALp : valid_path (Ctx C) [] p),
+  match read_snd ϕ t with
+  | Some t' =>
+    match pmap_snd ϕ p with
+    | Some p' =>
+      exists C', Some (Closure x e C') = read m' t' /\
+        valid_path (Ctx C') [] p'
     | None => False
-    end
-  | Ev (Ptr t) v (Ctx Cv) =>
-    exists ev, Some ev = read m t /\
-    match ev with
-    | Closure x e C =>
-      v = v_fn x e /\ C = Cv
-    end
-  | _ => False
+    end 
+  | None => False
   end.
 
-Definition avalid_edge `{Eq T} (m : memory T) (e : edge T) :=
-  match e with
-  | Ex (Ctx C) x (Ptr tx) =>
-    match addr_x C x with
-    | Some t => t = tx
-    | None => False
-    end
-  | EM (Ctx C) M (Ctx CM) =>
-    match ctx_M C M with
-    | Some C => C = CM
-    | None => False
-    end
-  | Ev (Ptr t) v (Ctx Cv) =>
-    exists ev, In ev (aread m t) /\
-    match ev with
-    | Closure x e C =>
-      v = v_fn x e /\ C = Cv
-    end
-  | _ => False
+Definition equiv_fst_ϕ_C `{Eq T} `{Eq TT} (ϕ : list (T * TT)) C C' :=
+  forall p
+    (VALp : valid_path (Ctx C) [] p),
+  match pmap_fst ϕ p with
+  | Some p' => valid_path (Ctx C') [] p'
+  | None => False
   end.
 
-Lemma same_valid_edge `{Eq T} :
-  forall e m m' (SAME : same m m')
-    (VALe : valid_edge m e),
-  valid_edge m' e.
-Proof.
-  ii. unfold valid_edge.
-  repeat des_goal; repeat des_hyp; clarify;
-  ss; repeat des_hyp; clarify.
-  des. repeat des_hyp; clarify.
-  des; clarify.
-  exists (Closure x e C). eauto.
-  unfold same in SAME.
-  rewrite <- SAME. eauto.
-Qed.
-
-Lemma asame_avalid_edge `{Eq T} :
-  forall e m m' (SAME : asame m m')
-    (VALe : avalid_edge m e),
-  avalid_edge m' e.
-Proof.
-  ii. unfold avalid_edge.
-  repeat des_goal; repeat des_hyp; clarify;
-  ss; repeat des_hyp; clarify.
-  des. repeat des_hyp; clarify.
-  des; clarify.
-  exists (Closure x e C). eauto.
-  unfold asame in SAME.
-  rewrite <- SAME. eauto.
-Qed.
-
-Fixpoint Edges `{Eq T} (n : node T) (p : path T) :=
-  match p with
-  | Pnil => []
-  | Px x n' tl => Ex n x n' :: Edges n' tl
-  | PM M n' tl => EM n M n' :: Edges n' tl
-  | Pv v n' tl => Ev n v n' :: Edges n' tl
+Definition equiv_snd_ϕ_C `{Eq T} `{Eq TT} (ϕ : list (T * TT)) C C' :=
+  forall p
+    (VALp : valid_path (Ctx C) [] p),
+  match pmap_snd ϕ p with
+  | Some p' => valid_path (Ctx C') [] p'
+  | None => False
   end.
 
-Lemma vpath_iff_vedge `{Eq T} :
-  forall p m n,
-    valid_path n m p <->
-    forall e (IN : In e (Edges n p)), valid_edge m e.
+Lemma equiv_fst_ϕ_aux `{Eq T} `{Eq TT} (ϕ : list (T * TT)) 
+  m m' (EQm : equiv_fst_ϕ_m ϕ m m') :
+  forall n C C' (EQC : equiv_fst_ϕ_C ϕ C C')
+    p (VALp : valid_path (Ctx C) m p)
+    (LE : plen p <= n),
+  match pmap_fst ϕ p with
+  | Some p' => valid_path (Ctx C') m' p'
+  | None => False
+  end.
 Proof.
-  induction p; ii; ss; repeat des_goal; repeat des_hyp; clarify; des;
-  split; ii; des; clarify; ltac:(
-  let HH := fresh "HH" in
-  match goal with
-  | H : forall e, Ex ?n ?x ?n' = e \/ _ -> _ |- _ =>
-    specialize (H (Ex n x n')) as HH; 
-    exploit HH; eauto;
-    ii; ss; repeat des_hyp; clarify
-  | H : forall e, EM ?n ?M ?n' = e \/ _ -> _ |- _ =>
-    specialize (H (EM n M n')) as HH; 
-    exploit HH; eauto;
-    ii; ss; repeat des_hyp; clarify
-  | H : forall e, Ev ?n ?v ?n' = e \/ _ -> _ |- _ =>
-    specialize (H (Ev n v n')) as HH; 
-    exploit HH; eauto;
-    ii; ss; repeat des_hyp; clarify
-  | _ => idtac
-  end).
-  - ss; des_goal; clarify.
-  - rewrite IHp in *. eauto.
-  - split; try rewrite IHp; ii; eauto.
-  - ss; des_goal; clarify.
-  - rewrite IHp in *. eauto.
-  - split; try rewrite IHp; ii; eauto.
-  - ss. exists ev. 
-    des_goal; des; repeat split; clarify.
+  unfold equiv_fst_ϕ_m in *.
+  unfold equiv_fst_ϕ_C in *.
+  induction n.
+  ii. destruct p; ss; nia.
+  ii; ss. destruct p; ss.
   - des_hyp; des; clarify.
-    rewrite IHp in *; eauto.
-  - des. exists ev.
-    des_goal; des; repeat split; clarify.
-    rewrite IHp; ii; eauto.
+    exploit (EQC (Px x t Pnil)). s. rw. eauto.
+    s. ii. repeat des_hyp; des; clarify.
+    ss. des_hyp; des; clarify.
+    destruct n; ss.
+    destruct p; ss; first [rw; eauto | nia].
+    destruct p; ss. rw. eauto.
+    des. des_hyp; des; clarify.
+    exploit (EQm t Pnil _ _ _); eauto.
+    ii. repeat des_hyp; des; clarify.
+    exploit (IHn C0 C'0 _ p); eauto.
+    ii.
+    exploit (EQm t p0); eauto. repeat rw.
+    ii. repeat des_hyp; des; clarify.
+    revert x3. rrw. ii. clarify. nia.
+    ii. des_hyp.
+    s. rw. split; eauto. eexists. split; eauto. s. eauto.
+  - des_hyp.
+    exploit (EQC (PM M Pnil)). s. rw. eauto.
+    ii. ss. des_hyp.
+    exploit (IHn d d0 _ p).
+    ii. exploit (EQC (PM M p0)). s. rw. eauto.
+    s. ii. repeat des_hyp; clarify.
+    revert x1. s. rw. eauto. eauto. nia.
+    ii. des_hyp. s. rw. eauto.
 Qed.
 
-Lemma avpath_iff_avedge `{Eq T} :
-  forall p m n,
-    avalid_path n m p <->
-    forall e (IN : In e (Edges n p)), avalid_edge m e.
+Lemma equiv_snd_ϕ_aux `{Eq T} `{Eq TT} (ϕ : list (T * TT)) 
+  m m' (EQm : equiv_snd_ϕ_m ϕ m m') :
+  forall n C C' (EQC : equiv_snd_ϕ_C ϕ C C')
+    p (VALp : valid_path (Ctx C) m p)
+    (LE : plen p <= n),
+  match pmap_snd ϕ p with
+  | Some p' => valid_path (Ctx C') m' p'
+  | None => False
+  end.
 Proof.
-  induction p; ii; ss; repeat des_goal; repeat des_hyp; clarify; des;
-  split; ii; des; clarify; ltac:(
-  let HH := fresh "HH" in
-  match goal with
-  | H : forall e, Ex ?n ?x ?n' = e \/ _ -> _ |- _ =>
-    specialize (H (Ex n x n')) as HH; 
-    exploit HH; eauto;
-    ii; ss; repeat des_hyp; clarify
-  | H : forall e, EM ?n ?M ?n' = e \/ _ -> _ |- _ =>
-    specialize (H (EM n M n')) as HH; 
-    exploit HH; eauto;
-    ii; ss; repeat des_hyp; clarify
-  | H : forall e, Ev ?n ?v ?n' = e \/ _ -> _ |- _ =>
-    specialize (H (Ev n v n')) as HH; 
-    exploit HH; eauto;
-    ii; ss; repeat des_hyp; clarify
-  | _ => idtac
-  end).
-  - ss; des_goal; clarify.
-  - rewrite IHp in *. eauto.
-  - split; try rewrite IHp; ii; eauto.
-  - ss; des_goal; clarify.
-  - rewrite IHp in *. eauto.
-  - split; try rewrite IHp; ii; eauto.
-  - ss. exists ev. 
-    des_goal; des; repeat split; clarify.
+  unfold equiv_snd_ϕ_m in *.
+  unfold equiv_snd_ϕ_C in *.
+  induction n.
+  ii. destruct p; ss; nia.
+  ii; ss. destruct p; ss.
   - des_hyp; des; clarify.
-    rewrite IHp in *; eauto.
-  - des. exists ev.
-    des_goal; des; repeat split; clarify.
-    rewrite IHp; ii; eauto.
-Qed.
-
-Definition reachable `{Eq T} root m e :=
-  exists p,
-    valid_path root m p /\
-    In e (Edges root p).
-
-Definition lvertex `{Eq T} (e : edge T) :=
-  match e with
-  | Ex n _ _
-  | EM n _ _
-  | Ev n _ _ => n
-  end.
-
-Definition rvertex `{Eq T} (e : edge T) :=
-  match e with
-  | Ex _ _ n
-  | EM _ _ n
-  | Ev _ _ n => n
-  end.
-
-Lemma paste_vpath `{Eq T} :
-  forall n m e (REACH : reachable n m e) e'
-    (REACH' : reachable (rvertex e) m e'),
-  reachable n m e'.
-Proof.
-  ii. destruct REACH as [p [VAL IN]].
-  ginduction p; ii; ss; repeat des_hyp; des; clarify; ss.
-  - destruct REACH' as [p' [VAL' IN']].
-    exists (Px x (Ptr t0) p').
-    ss. rw. eauto.
-  - exploit IHp; eauto. intros REACH.
-    destruct REACH as [p' [VAL' IN']].
-    exists (Px x (Ptr t0) p').
-    ss. rw. eauto.
-  - destruct REACH' as [p' [VAL' IN']].
-    exists (PM M (Ctx d) p').
-    ss. rw. eauto.
-  - exploit IHp; eauto. intros REACH.
-    destruct REACH as [p' [VAL' IN']].
-    exists (PM M (Ctx d) p').
-    ss. rw. eauto.
-  - des_hyp; des; clarify.
-    destruct REACH' as [p' [VAL' IN']].
-    exists (Pv (v_fn x e) (Ctx C0) p').
-    ss. split; eauto.
-    exists (Closure x e C0). eauto.
-  - des_hyp; des; clarify.
-    exploit IHp; eauto. intros REACH.
-    destruct REACH as [p' [VAL' IN']].
-    exists (Pv (v_fn x e0) (Ctx C0) p').
-    ss. split; eauto.
-    exists (Closure x e0 C0). eauto.
-Qed.
-
-Lemma reachable_left `{Eq T} :
-  forall n m e (REACH : reachable n m e),
-    n = lvertex e \/
-    exists e', reachable n m e' /\ rvertex e' = lvertex e.
-Proof.
-  ii. unfold reachable in REACH. des.
-  ginduction p; ii; ss; repeat des_hyp; clarify;
-  des; clarify; ss; repeat des_hyp;
-  clarify; des; clarify; eauto;
-  exploit IHp; eauto; ii; des; clarify; right.
-  - exists (Ex (Ctx C) x (Ptr t0)).
-    split; ss.
-    exists (Px x (Ptr t0) Pnil). ss. repeat rw. eauto.
-  - exists e'.
-    split; ss.
-    unfold reachable in *. des.
-    exists (Px x (Ptr t0) p0).
-    ss. rw. eauto.
-  - exists (EM (Ctx C0) M (Ctx d)).
-    split; ss.
-    exists (PM M (Ctx d) Pnil). ss. repeat rw. eauto.
-  - exists e'.
-    split; ss.
-    unfold reachable in *. des.
-    exists (PM M (Ctx d) p0).
-    ss. rw. eauto.
-  - exists (Ev (Ptr t) (v_fn x e0) (Ctx C0)).
-    split; ss.
-    exists (Pv (v_fn x e0) (Ctx C0) Pnil). ss.
-    repeat split; eauto.
-    exists (Closure x e0 C0). ss.
-  - exists e'.
-    split; ss.
-    unfold reachable in *. des.
-    exists (Pv (v_fn x e0) (Ctx C0) p0).
-    ss. split; eauto.
-    exists (Closure x e0 C0). ss.
-Qed.
-
-Lemma reachable_eq_def `{Eq T} :
-  forall n m e,
-    reachable n m e <->
-    (valid_edge m e /\
-      (n = lvertex e \/
-      exists e', 
-        reachable n m e' /\
-        rvertex e' = lvertex e)).
-Proof.
-  ii. split; intros REACH; des; clarify.
-  - split. unfold reachable in *. des.
-    rewrite vpath_iff_vedge in REACH. eauto.
-    apply reachable_left. eauto.
-  - destruct e; ss; repeat des_hyp; clarify; des;
-    repeat des_hyp; des; clarify;
-    match goal with
-    | |- context [Ex _ ?x (Ptr ?t)] =>
-      exists (Px x (Ptr t) Pnil)
-    | |- context [EM _ ?M (Ctx ?C)] =>
-      exists (PM M (Ctx C) Pnil)
-    | |- context [Ev _ ?v (Ctx ?C)] =>
-      exists (Pv v (Ctx C) Pnil)
-    end; ss; try rw; eauto.
-    split; eauto.
-    exists (Closure x e C). eauto.
-  - eapply paste_vpath; eauto.
-    rw. destruct e; ss; repeat des_hyp; des; clarify.
-    exists (Px x (Ptr t) Pnil). ss. rw. eauto.
-    exists (PM M (Ctx C0) Pnil). ss. rw. eauto.
-    des_hyp; des; clarify.
-    exists (Pv (v_fn x e) (Ctx C) Pnil). ss.
-    split; eauto.
-    exists (Closure x e C). eauto.
-Qed.
-
-Fixpoint remove_t `{Eq T} (m : memory T) t :=
-  match m with
-  | [] => []
-  | (t', v) :: tl =>
-    let tl := remove_t tl t in
-    if eqb t t' then tl else (t', v) :: tl
-  end.
-
-Fixpoint reach_C `{Eq T} seenx seenM (Cout Cin : dy_ctx T) :=
-  match Cin with
-  | [||] => []
-  | dy_binde x t Cin =>
-    if Inb x seenx then reach_C seenx seenM Cout Cin
-    else Ex (Ctx Cout) x (Ptr t) ::
-    reach_C (x :: seenx) seenM Cout Cin
-  | dy_bindm M Cout' Cin =>
-    if Inb M seenM then reach_C seenx seenM Cout Cin
-    else reach_C [] [] Cout' Cout' ++ 
-    EM (Ctx Cout) M (Ctx Cout') ::
-    reach_C seenx (M :: seenM) Cout Cin
-  end.
-
-Fixpoint InL `{Eq T} (n : node T) (l : list (edge T)) :=
-  match l with
-  | [] => false
-  | e :: tl => eqb n (lvertex e) || InL n tl
-  end.
-
-Fixpoint InR `{Eq T} (n : node T) (l : list (edge T)) :=
-  match l with
-  | [] => false
-  | e :: tl => eqb n (rvertex e) || InR n tl
-  end.
-
-Lemma InL_In `{Eq T} :
-  forall l n, InL n l = true <-> exists e, In e l /\ n = lvertex e.
-Proof.
-  induction l; ii; ss; split; ii; 
-  repeat des_goal; repeat des_hyp; ss; des; clarify;
-  first [rewrite eq_node_eq in * | rewrite eq_node_neq in *];
-  clarify.
-  - exists a. eauto.
-  - rewrite IHl in *. des. clarify.
-    exists e. eauto.
-  - rewrite IHl. exists e. eauto.
-Qed.
-
-Lemma InL_nIn `{Eq T} :
-  forall l n, InL n l = false <-> forall e, ~ In e l \/ n <> lvertex e.
-Proof.
-  split; intros NIN.
-  - assert (InL n l <> true) as HINT.
-    { refl_bool. eauto. }
-    red in HINT. rewrite InL_In in HINT.
+    exploit (EQC (Px x t Pnil)). s. rw. eauto.
+    s. ii. repeat des_hyp; des; clarify.
+    ss. des_hyp; des; clarify.
+    destruct n; ss.
+    destruct p; ss; first [rw; eauto | nia].
+    destruct p; ss. rw. eauto.
+    des. des_hyp; des; clarify.
+    exploit (EQm t Pnil _ _ _); eauto.
+    ii. repeat des_hyp; des; clarify.
+    exploit (IHn C0 C'0 _ p); eauto.
     ii.
-    destruct (Inb e l) eqn:CASEIn;
-    destruct (eqb n (lvertex e)) eqn:CASEv;
-    try rewrite Inb_eq in *;
-    try rewrite eqb_eq in *;
-    try rewrite Inb_neq in *;
-    try rewrite eqb_neq in *;
-    clarify; eauto.
-    exfalso. apply HINT. exists e. eauto.
-  - refl_bool. ii.
-    rewrite InL_In in *. des.
-    specialize (NIN e). des; eauto.
+    exploit (EQm t p0); eauto. repeat rw.
+    ii. repeat des_hyp; des; clarify.
+    revert x3. rrw. ii. clarify. nia.
+    ii. des_hyp.
+    s. rw. split; eauto. eexists. split; eauto. s. eauto.
+  - des_hyp.
+    exploit (EQC (PM M Pnil)). s. rw. eauto.
+    ii. ss. des_hyp.
+    exploit (IHn d d0 _ p).
+    ii. exploit (EQC (PM M p0)). s. rw. eauto.
+    s. ii. repeat des_hyp; clarify.
+    revert x1. s. rw. eauto. eauto. nia.
+    ii. des_hyp. s. rw. eauto.
 Qed.
 
-Lemma InR_In `{Eq T} :
-  forall l n, InR n l = true <-> exists e, In e l /\ n = rvertex e.
-Proof.
-  induction l; ii; ss; split; ii; 
-  repeat des_goal; repeat des_hyp; ss; des; clarify;
-  first [rewrite eq_node_eq in * | rewrite eq_node_neq in *];
-  clarify.
-  - exists a. eauto.
-  - rewrite IHl in *. des. clarify.
-    exists e. eauto.
-  - rewrite IHl. exists e. eauto.
-Qed.
+Inductive fix_result `{Eq T} `{Eq TT} :=
+  | Fix (m mbot : memory T) (m' : memory TT) (ϕ : list (T * TT)) (tϕ : TT)
+  | Unfix
+.
 
-Lemma InR_nIn `{Eq T} :
-  forall l n, InR n l = false <-> forall e, ~ In e l \/ n <> rvertex e.
-Proof.
-  split; intros NIN.
-  - assert (InR n l <> true) as HINT.
-    { refl_bool. eauto. }
-    red in HINT. rewrite InR_In in HINT.
-    ii.
-    destruct (Inb e l) eqn:CASEIn;
-    destruct (eqb n (rvertex e)) eqn:CASEv;
-    try rewrite Inb_eq in *;
-    try rewrite eqb_eq in *;
-    try rewrite Inb_neq in *;
-    try rewrite eqb_neq in *;
-    clarify; eauto.
-    exfalso. apply HINT. exists e. eauto.
-  - refl_bool. ii.
-    rewrite InR_In in *. des.
-    specialize (NIN e). des; eauto.
-Qed.
-
-Lemma InL_app_iff `{Eq T} :
-  forall n l1 l2,
-  InL n (l1 ++ l2) = true <-> InL n l1 = true \/ InL n l2 = true.
-Proof.
-  ii. split; ii; rewrite InL_In in *; des; clarify.
-  - rewrite in_app_iff in *. des.
-    left. exists e. eauto.
-    right. rewrite InL_In. exists e. eauto.
-  - exists e. rewrite in_app_iff. eauto.
-  - rewrite InL_In in *. des.
-    exists e. rewrite in_app_iff. eauto.
-Qed.
-
-Lemma InR_app_iff `{Eq T} :
-  forall n l1 l2,
-  InR n (l1 ++ l2) = true <-> InR n l1 = true \/ InR n l2 = true.
-Proof.
-  ii. split; ii; rewrite InR_In in *; des; clarify.
-  - rewrite in_app_iff in *. des.
-    left. exists e. eauto.
-    right. rewrite InR_In. exists e. eauto.
-  - exists e. rewrite in_app_iff. eauto.
-  - rewrite InR_In in *. des.
-    exists e. rewrite in_app_iff. eauto.
-Qed.
-
-Fixpoint reach_m_step `{Eq T} acc (m : memory T) :=
-  match m with
-  | [] => (acc, [])
-  | (t, v) :: m =>
-    if InR (Ptr t) acc then match v with
-    | Closure x e C =>
-      (reach_C [] [] C C ++ 
-      Ev (Ptr t) (v_fn x e) (Ctx C) ::
-      acc, remove_t m t)
-    end else match reach_m_step acc m with
-    | (acc, m) => (acc, (t, v) :: m)
+Fixpoint trans_iso_m_aux `{Eq TT} `{Eq aTT} `{TotalOrder T} `{Eq aT}
+  (α' : TT -> aTT) (inv_α : (T * aT) -> T) φ φ'
+  (ϕ : list (TT * T)) (tϕ : T)
+  (am : memory aT) (m1 : memory T) (m2 m : memory TT) fuel :=
+  match trans_m_step α' inv_α φ φ' ϕ tϕ am m with
+  | Unchanged => Fix m2 m m1 ϕ tϕ
+  | Changed t' v' t v ϕ' tϕ' =>
+    let m1' := (t, v) :: m1 in
+    let m2' := (t', v') :: m2 in
+    let m' := remove_t m t' in
+    match fuel with
+    | 0 => Unfix
+    | S fuel' => trans_iso_m_aux α' inv_α φ φ' ϕ' tϕ' am m1' m2' m' fuel'
     end
+  | Failed => Unfix
   end.
 
-Fixpoint areach_m_step `{Eq T} acc (m : memory T) :=
-  match m with
-  | [] => (acc, [])
-  | (t, v) :: m =>
-    if InR (Ptr t) acc then match v with
-    | Closure x e C =>
-      match areach_m_step acc m with
-      | (acc, m) =>
-        (reach_C [] [] C C ++
-        Ev (Ptr t) (v_fn x e) (Ctx C) ::
-        acc, m)
-      end
-    end else match areach_m_step acc m with
-    | (acc, m) => (acc, (t, v) :: m)
-    end
-  end.
+Definition trans_iso_m `{Eq TT} `{Eq aTT} `{TotalOrder T} `{Eq aT}
+  (α' : TT -> aTT) (inv_α : (T * aT) -> T) φ φ'
+  (ϕ : list (TT * T)) (tϕ : T)
+  (am : memory aT) (m : memory TT) :=
+  trans_iso_m_aux α' inv_α φ φ' ϕ tϕ am [] [] m (length m).
 
-Fixpoint reach_m_aux `{Eq T} acc (m : memory T) fuel :=
-  match reach_m_step acc m with
-  | (acc, m') =>
-    if Nat.eqb (List.length m) (List.length m') then
-      Some acc
-    else match fuel with
-    | 0 => None
-    | S fuel => reach_m_aux acc m' fuel
-    end
-  end.
+Definition trans_iso_m_pre `{Eq TT} `{Eq aTT} `{TotalOrder T} `{Eq aT}
+  (α' : TT -> aTT) (inv_α : (T * aT) -> T) (α : T -> aT) φ φ'
+  (ϕ : list (TT * T)) (tϕ : T) (C2 : dy_ctx TT) (C1 : dy_ctx T)
+  (am : memory aT) (m1 : memory T) (m2 m : memory TT) :=
+  (forall t, None <> read m2 t -> None = read m t) /\
+  (forall t, reachable (Ctx C2) m2 t <-> None <> read_fst ϕ t) /\
+  equiv_fst_ϕ_C ϕ C2 C1 /\
+  equiv_snd_ϕ_C ϕ C1 C2 /\
+  equiv_fst_ϕ_m ϕ m2 m1 /\
+  equiv_snd_ϕ_m ϕ m1 m2 /\
+  ϕ_spec α' α φ φ' ϕ tϕ /\
+  inv_α_spec α inv_α /\
+  aIso (Ctx (trans_C α' C2)) (trans_m α' (m2 ++ m))
+       (Ctx (trans_C α C1)) am φ φ' /\
+  (forall t v, Some v = read m1 t ->
+    In (trans_v α v) (aread am (α t)))
+.
 
-Lemma remove_t_dec `{Eq T} :
-  forall (m : memory T) t,
-  (List.length (remove_t m t)) <= (List.length m).
+Lemma pre_implies_pre `{Eq TT} `{Eq aTT} `{TotalOrder T} `{Eq aT}
+  (α' : TT -> aTT) (inv_α : (T * aT) -> T) (α : T -> aT) φ φ'
+  (ϕ : list (TT * T)) (tϕ : T) (C2 : dy_ctx TT) (C1 : dy_ctx T)
+  (am : memory aT) (m1 : memory T) (m2 m : memory TT) :
+  trans_iso_m_pre α' inv_α α φ φ' ϕ tϕ C2 C1 am m1 m2 m ->
+  trans_m_step_pre α' φ φ' ϕ am m.
 Proof.
-  induction m; intros; simpl; eauto.
-  repeat des_goal; repeat des_hyp; clarify;
-  try rewrite eqb_eq in *; subst;
-  match goal with
-  | |- context [remove_t _ ?t] =>
-    specialize (IHm t); nia
-  end.
-Qed.
-
-Lemma remove_t_read `{Eq T} :
-  forall (m : memory T) t,
-  None = read (remove_t m t) t.
-Proof.
-  induction m; ii; ss; repeat des_goal; repeat des_hyp; clarify.
-  rewrite eqb_eq in *; clarify. rewrite t_refl in *. clarify.
-Qed.
-
-Lemma remove_t_read_some `{Eq T} :
-  forall (m : memory T) t t' (NEQ : t <> t'),
-  read (remove_t m t) t' = read m t'.
-Proof.
-  induction m; ii; ss; repeat des_goal; repeat des_hyp;
-  try rewrite eqb_eq in *; clarify; eauto.
-Qed.
-
-Lemma reach_m_step_dec `{Eq T} :
-  forall m acc,
-  match reach_m_step acc m with
-  | (_, m') => length m' <= length m
-  end.
-Proof.
-  induction m; ii; ss;
-  repeat des_goal; repeat des_hyp; clarify; ss.
-  - pose proof (remove_t_dec m t). nia.
-  - specialize (IHm acc). repeat des_hyp; clarify. nia.
-Qed.
-
-Lemma areach_m_step_dec `{Eq T} :
-  forall (m : memory T) acc,
-  match areach_m_step acc m with
-  | (_, m') => length m' <= length m
-  end.
-Proof.
-  induction m; intros; simpl; eauto;
-  repeat des_goal; repeat des_hyp; clarify; simpl.
-  - specialize (IHm acc). 
-    repeat des_hyp; clarify. auto.
-  - specialize (IHm acc).
-    repeat des_hyp; clarify. nia.
-Qed.
-
-Lemma reach_m_step_same `{Eq T} :
-  forall m acc,
-  match reach_m_step acc m with
-  | (acc', m') =>
-    if length m =? length m' then
-      acc = acc' /\ m = m'
-    else True
-  end.
-Proof.
-  induction m; ii; ss; repeat des_goal; repeat des_hyp; des; clarify;
-  rewrite Nat.eqb_eq in *; clarify.
-  - pose proof (reach_m_step_dec m acc).
-    pose proof (remove_t_dec m t).
-    repeat des_hyp; clarify. nia.
-  - ss.
-    assert (length m = length l2) as RR. nia.
-    rewrite <- Nat.eqb_eq in RR.
-    specialize (IHm acc).
-    repeat des_hyp; clarify; des; clarify.
-Qed.
-
-Fixpoint areach_m_aux `{Eq T} acc (m : memory T) fuel :=
-  match areach_m_step acc m with
-  | (acc, m') =>
-    if Nat.eqb (List.length m) (List.length m') then
-      Some acc
-    else match fuel with
-    | 0 => None
-    | S fuel => areach_m_aux acc m' fuel
-    end
-  end.
-
-Definition reach_m `{Eq T} init (m : memory T) :=
-  reach_m_aux init m (List.length m).
-
-Definition areach_m `{Eq T} init (m : memory T) :=
-  areach_m_aux init m (List.length m).
-
-Lemma reach_m_aux_some `{Eq T} :
-  forall fuel m init (GE : (List.length m) <= fuel),
-    exists reached, reach_m_aux init m fuel = Some reached.
-Proof.
-  induction fuel; intros; destruct m; simpl in *; eauto;
-  try (inversion GE; fail).
-  assert (List.length m <= fuel). { nia. }
-  repeat des_goal; repeat des_hyp; clarify; eauto; apply IHfuel;
-  match goal with
-  | _ : context [remove_t ?m ?t] |- _ =>
-    pose proof (remove_t_dec m t);
-    repeat des_hyp; ss; clarify; try nia
-  | _ : context [reach_m_step ?init ?m] |- _ =>
-    pose proof (reach_m_step_dec m init);
-    repeat des_hyp; ss; clarify
-  end.
-  - rewrite Nat.eqb_neq in *. nia.
-Qed.
-
-Lemma areach_m_aux_some `{Eq T} :
-  forall fuel m init (GE : (List.length m) <= fuel),
-    exists reached, areach_m_aux init m fuel = Some reached.
-Proof.
-  induction fuel; intros; destruct m; simpl in *; eauto;
-  try (inversion GE; fail).
-  assert (List.length m <= fuel). { nia. }
-  repeat des_goal; repeat des_hyp; clarify; eauto; apply IHfuel;
-  match goal with
-  | _ => rw; nia
-  | _ =>
-    pose proof (areach_m_step_dec m init);
-    repeat des_hyp; ss; clarify;
-    rewrite Nat.eqb_neq in *; nia
-  end.
-Qed.
-
-Lemma relax_fuel `{Eq T} :
-  forall fuel fuel' (LE : fuel' <= fuel) init m reached
-    (EV : reach_m_aux init m fuel' = Some reached),
-  reach_m_aux init m fuel = Some reached.
-Proof.
-  induction fuel;
-  ii; inv LE; ss; repeat des_goal; repeat des_hyp; clarify;
-  apply IHfuel in EV; eauto.
-  - rewrite <- EV. symmetry.
-    eapply IHfuel; eauto.
-    destruct fuel'; ss; repeat rw; eauto.
-  - destruct fuel; ss; repeat des_hyp; clarify.
-    apply IHfuel with (fuel' := fuel); eauto.
-Qed.
-
-Lemma arelax_fuel `{Eq T} :
-  forall fuel fuel' (LE : fuel' <= fuel) init m reached
-    (EV : areach_m_aux init m fuel' = Some reached),
-  areach_m_aux init m fuel = Some reached.
-Proof.
-  induction fuel;
-  ii; inv LE; ss; repeat des_goal; repeat des_hyp; clarify;
-  apply IHfuel in EV; eauto.
-  - rewrite <- EV. symmetry.
-    eapply IHfuel; eauto.
-    destruct fuel'; ss; repeat rw; eauto.
-  - destruct fuel; ss; repeat des_hyp; clarify.
-    apply IHfuel with (fuel' := fuel); eauto.
-Qed.
-
-Lemma reach_m_some `{Eq T} :
-  forall m init, exists reached, reach_m init m = Some reached.
-Proof.
-  intros. unfold reach_m. apply reach_m_aux_some. eauto.
-Qed.
-
-Lemma areach_m_some `{Eq T} :
-  forall m init, exists reached, areach_m init m = Some reached.
-Proof.
-  intros. unfold areach_m. apply areach_m_aux_some. eauto.
-Qed.
-
-Definition reach `{Eq T} (n : node T) (m : memory T) :=
-  match n with
-  | Ctx C => reach_m (reach_C [] [] C C) m
-  | Ptr t =>
-    let init := match read m t with
-    | Some (Closure x e C) => 
-      (Ev (Ptr t) (v_fn x e) (Ctx C)) ::
-      reach_C [] [] C C
-    | None => []
-    end in
-    reach_m init (remove_t m t)
-  end.
-
-Fixpoint flatten {T} (ll : list (list T)) :=
-  match ll with
-  | [] => []
-  | l :: tll => l ++ flatten tll
-  end.
-
-Definition areach `{Eq T} (n : node T) (m : memory T) :=
-  match n with
-  | Ctx C => areach_m (reach_C [] [] C C) m
-  | Ptr t => 
-    let init := flatten (map (fun v => match v with
-    | Closure x e C => 
-      (Ev (Ptr t) (v_fn x e) (Ctx C)) ::
-      reach_C [] [] C C
-    end) (aread m t)) in
-    areach_m init (remove_t m t)
-  end.
-
-Fixpoint memify `{Eq T} (edges : list (edge T)) : memory T :=
-  match edges with
-  | [] => []
-  | Ev (Ptr t) (v_fn x e) (Ctx C) :: tl =>
-    (t, Closure x e C) :: memify tl
-  | _ :: tl => memify tl
-  end.
-
-Lemma app_memify `{Eq T} :
-  forall l1 l2,
-    memify (l1 ++ l2) = memify l1 ++ memify l2.
-Proof.
-  induction l1; ii; ss;
-  repeat des_goal; repeat des_hyp; clarify.
-  rw. reflexivity.
-Qed.
-
-Lemma valid_edge_C `{Eq T} :
-  forall e m C (LEFT : Ctx C = lvertex e),
-  valid_edge m e <-> valid_edge [] e.
-Proof.
-  ii. destruct e; ss; repeat des_goal; repeat des_hyp; clarify.
-Qed.
-
-Definition reach_C_pre `{Eq T} seenx seenM (Cout Cin : dy_ctx T) :=
-  (forall x (NIN : ~ In x seenx),
-    match addr_x Cout x, addr_x Cin x with
-    | Some tx, Some tx' => tx = tx'
-    | None, None => True
-    | _, _ => False
-    end) /\
-  (forall M (NIN : ~ In M seenM),
-    match ctx_M Cout M, ctx_M Cin M with
-    | Some CM, Some CM' => CM = CM'
-    | None, None => True
-    | _, _ => False
-    end).
-
-Definition reach_C_post `{Eq T} seenx seenM Cout res :=
-  (forall x (NIN : ~ In x seenx),
-  match addr_x Cout x with
-  | Some t => In (Ex (Ctx Cout) x (Ptr t)) res
-  | None => True
-  end) /\
-  (forall M (NIN : ~ In M seenM),
-  match ctx_M Cout M with
-  | Some CM => In (EM (Ctx Cout) M (Ctx CM)) res
-  | None => True
-  end) /\
-  (forall C e e'
-    (IN : In e res)
-    (RIGHT : Ctx C = rvertex e)
-    (LEFT : Ctx C = lvertex e')
-    (VAL : valid_edge [] e'),
-    In e' res) /\
-  (forall e (IN : In e res),
-    valid_edge [] e) /\
-  (forall e C
-    (IN : In e res) 
-    (LEFT : Ctx C = lvertex e),
-    C = Cout \/
-    exists e', Ctx C = rvertex e' /\ In e' res).
-
-Lemma reach_C_pre_post `{Eq T} :
-  forall Cin Cout seenx seenM
-    (INV : reach_C_pre seenx seenM Cout Cin),
-  reach_C_post seenx seenM Cout (reach_C seenx seenM Cout Cin).
-Proof.
-  induction Cin; ii; ss;
-  unfold reach_C_pre in *;
-  unfold reach_C_post in *;
-  des;
-  repeat match goal with
-  | |- _ /\ _ => split
-  end; ii; ss;
-  repeat des_goal; repeat des_hyp; clarify.
-  - exploit INV; eauto. rw. eauto.
-  - exploit INV0; eauto. rw. eauto.
-  - rewrite Inb_eq in *.
-    exploit INV; eauto. rw.
-    ii; repeat des_hyp; clarify.
-    rewrite eqb_ID_eq in *; clarify.
-    exploit (IHCin Cout seenx seenM).
-    split; eauto.
-    ii. exploit (INV x1); eauto.
-    ii; repeat des_hyp; clarify.
-    rewrite eqb_ID_eq in *. clarify.
-    rw. eauto. rw. eauto.
-    ii. des.
-    specialize (x2 x0 NIN).
-    repeat des_hyp; clarify.
-  - rewrite Inb_neq in *.
-    specialize (INV x0 NIN) as HINT.
-    rewrite GDES in *.
-    repeat des_hyp; clarify.
-    rewrite eqb_ID_eq in *; clarify; eauto.
-    right.
-    exploit (IHCin Cout (x :: seenx) seenM).
-    split; eauto.
-    ii. exploit (INV x1).
-    red; ii; ss; eauto.
-    ii. repeat des_hyp; clarify.
-    rewrite eqb_ID_eq in *. ss. clarify. contradict.
-    rw. eauto. rw. eauto.
-    ii. des. exploit (x2 x0).
-    red; ii; ss; des; clarify.
-    rewrite eqb_ID_neq in *. eauto.
-    ii. repeat des_hyp; clarify.
-  - rewrite Inb_eq in *.
-    exploit (IHCin Cout seenx seenM).
-    split; eauto.
-    ii. exploit INV; eauto.
-    ii; repeat des_hyp; clarify.
-    rewrite eqb_ID_eq in *. clarify.
-    rw. eauto. rw. eauto.
-    ii; des.
-    specialize (x0 M NIN).
-    rewrite GDES in *. eauto.
-  - right. rewrite Inb_neq in *.
-    exploit (IHCin Cout (x :: seenx) seenM).
-    split; eauto.
-    ii. exploit (INV x0).
-    red; ii; ss; eauto.
-    ii. repeat des_hyp; clarify.
-    rewrite eqb_ID_eq in *. clarify. ss. contradict.
-    rw. eauto. rw. eauto.
-    ii. des. exploit (x0 M); eauto.
-    rw. eauto.
-  - rewrite Inb_eq in *.
-    specialize (IHCin Cout seenx seenM).
-    exploit IHCin; eauto.
-    split; eauto.
-    ii. exploit INV; eauto.
-    ii; repeat des_hyp; clarify.
-    rewrite eqb_ID_eq in *; clarify.
-    rw. eauto. rw. eauto.
-    ii; des. eauto.
-  - ss. des; clarify.
-    rewrite Inb_neq in *.
-    exploit (IHCin Cout (x :: seenx) seenM).
-    split; eauto.
-    ii. exploit (INV x0); eauto.
-    red; ii. apply NIN; ss; eauto.
-    ii. repeat des_hyp; clarify.
-    rewrite eqb_ID_eq in *; clarify.
-    ss; contradict.
-    rw. eauto. rw. eauto.
-    ii. des. eauto.
-  - rewrite Inb_eq in *.
-    exploit (IHCin Cout seenx seenM).
-    split; eauto.
-    ii. exploit INV; eauto.
-    ii; repeat des_hyp; clarify.
-    rewrite eqb_ID_eq in *; clarify.
-    rw. eauto. rw. eauto.
-    ii. des. eauto.
-  - rewrite Inb_neq in *.
-    des; clarify; ss.
-    + exploit INV; eauto.
-      ii. repeat des_hyp; try rewrite eqb_ID_neq in *; clarify.
-    + exploit (IHCin Cout (x :: seenx) seenM).
-      split; eauto.
-      ii. exploit (INV x0); eauto.
-      ii; ss; eauto.
-      ii. repeat des_hyp; clarify.
-      rewrite eqb_ID_eq in *. clarify. ss; contradict.
-      rw. eauto. rw. eauto.
-      ii. des. eauto.
-  - rewrite Inb_eq in *.
-    exploit (IHCin Cout seenx seenM); eauto.
-    split; eauto.
-    ii. exploit (INV x0); eauto.
-    ii; repeat des_hyp; clarify.
-    rewrite eqb_ID_eq in *; clarify.
-    rw. eauto. rw. eauto.
-    ii. des. eauto.
-  - rewrite Inb_neq in *.
-    ss; des; clarify; ss; clarify; eauto.
-    exploit (IHCin Cout (x :: seenx) seenM); eauto.
-    split; eauto.
-    ii. exploit (INV x0).
-    red; ii; ss; eauto.
-    ii; repeat des_hyp; clarify.
-    rewrite eqb_ID_eq in *; clarify. ss; contradict.
-    rw. eauto. rw. eauto.
-    ii. des. exploit x4; eauto.
-    ii. des; clarify; eauto.
-  - rewrite Inb_eq in *.
-    exploit (IHCin2 Cout seenx seenM).
-    split; eauto.
-    ii. exploit INV0; eauto.
-    ii; repeat des_hyp; clarify.
-    rewrite eqb_ID_eq in *; clarify.
-    rw. eauto. rw. eauto.
-    ii. des. exploit x1; eauto. rw. eauto.
-  - rewrite Inb_neq in *.
-    rewrite in_app_iff. right. right.
-    exploit (IHCin2 Cout seenx (M :: seenM)).
-    split; eauto.
-    ii. exploit (INV0 M0); eauto.
-    red; ii. ss; eauto.
-    ii; repeat des_hyp; clarify.
-    rewrite eqb_ID_eq in *; ss. contradict.
-    rw. eauto. rw. eauto.
-    ii. des.
-    exploit x1; eauto. rw. eauto.
-  - rewrite Inb_eq in *.
-    exploit (IHCin2 Cout seenx seenM).
-    split; eauto.
-    ii. exploit (INV0 M1); eauto.
-    ii; repeat des_hyp; clarify.
-    rewrite eqb_ID_eq in *; ss; clarify.
-    rw. eauto. rw. eauto.
-    ii. des. exploit (x1 M0); eauto.
-    rw. eauto.
-  - rewrite Inb_neq in *.
-    specialize (INV0 M0 NIN) as HINT.
-    rewrite GDES in HINT.
-    repeat des_hyp; clarify.
-    rewrite eqb_ID_eq in *; clarify.
-    rewrite in_app_iff. right. left. eauto.
-    rewrite eqb_ID_neq in *.
-    exploit (IHCin2 Cout seenx (M :: seenM)).
-    split; eauto.
-    ii. exploit (INV0 M1); eauto.
-    red; ii; ss; eauto.
-    ii; repeat des_hyp; clarify.
-    rewrite eqb_ID_eq in *; ss; clarify. contradict.
-    rw. eauto. rw. eauto.
-    ii. des. exploit (x1 M0); eauto.
-    red; ii; ss; des; clarify.
-    ii; repeat des_hyp; clarify.
-    rewrite in_app_iff. right. right. assumption.
-  - rewrite Inb_eq in *.
-    exploit (IHCin2 Cout seenx seenM).
-    split; eauto.
-    ii. exploit INV0; eauto.
-    ii; repeat des_hyp; clarify.
-    rewrite eqb_ID_eq in *; clarify.
-    rw. eauto. rw. eauto.
-    ii. des. eauto.
-  - rewrite Inb_neq in *.
-    rewrite in_app_iff in *. ss. des; clarify; ss; clarify.
-    + left. specialize (IHCin1 Cin1 [] []).
-      exploit IHCin1.
-      split; ii; ss; repeat des_goal; repeat des_hyp; clarify.
-      ii; des. eauto.
-    + left. specialize (IHCin1 Cin1 [] []).
-      destruct e'; ss; repeat des_hyp; clarify;
-      exploit IHCin1;
-      match goal with
-      | |- _ /\ _ =>
-        split; ii; ss; repeat des_goal; repeat des_hyp; clarify
-      | _ => ii; des
-      end.
-      exploit x1; eauto. rw. eauto.
-      exploit x1; eauto. rw. eauto.
-    + right. right.
-      specialize (IHCin2 Cout seenx (M :: seenM)).
-      exploit IHCin2.
-      split; eauto.
-      ii. exploit (INV0 M0); eauto.
-      red; ii; ss; eauto.
-      ii; repeat des_hyp; clarify.
-      rewrite eqb_ID_eq in *; ss; clarify. contradict.
-      rw. eauto. rw. eauto.
-      ii. des. eauto.
-  - rewrite Inb_eq in *.
-    exploit (IHCin2 Cout seenx seenM).
-    split; eauto.
-    ii. exploit INV0; eauto.
-    ii; repeat des_hyp; clarify.
-    rewrite eqb_ID_eq in *; clarify.
-    rw. eauto. rw. eauto.
-    ii. des. eauto.
-  - rewrite Inb_neq in *.
-    rewrite in_app_iff in *. ss.
-    des; clarify.
-    + exploit (IHCin1 Cin1 [] []).
-      split; ii; ss;
-      repeat des_goal; repeat des_hyp; clarify.
-      ii; des. eauto.
-    + exploit INV0; eauto.
-      ii. repeat des_hyp; clarify.
-      ss. rw. eauto.
-      rewrite eqb_ID_neq in *. contradict.
-      rewrite eqb_ID_neq in *. contradict.
-    + exploit (IHCin2 Cout seenx (M :: seenM)).
-      split; eauto.
-      ii. exploit (INV0 M0); eauto.
-      red; ii; ss; eauto.
-      ii; repeat des_hyp; clarify.
-      rewrite eqb_ID_eq in *; ss; clarify. contradict.
-      rw. eauto. rw. eauto.
-      ii. des. eauto.
-  - rewrite Inb_eq in *.
-    exploit (IHCin2 Cout seenx seenM).
-    split; eauto.
-    ii. exploit (INV0 M0); eauto.
-    ii. repeat des_hyp; clarify.
-    rewrite eqb_ID_eq in *; clarify.
-    rw. eauto. rw. eauto.
-    ii. des. eauto.
-  - rewrite Inb_neq in *.
-    rewrite in_app_iff in *. ss.
-    des; clarify.
-    + exploit (IHCin1 Cin1 [] []).
-      split; ii; repeat des_goal; repeat des_hyp; clarify.
-      ii. des.
-      exploit (INV0 M); eauto.
-      ii. repeat des_hyp; clarify;
-      try rewrite eqb_ID_neq in *; try contradict.
-      exploit x4; eauto.
-      ii. des; clarify.
-      * right. exists (EM (Ctx Cout) M (Ctx d0)).
-        split; ss. rewrite in_app_iff; ss. eauto.
-      * right. exists e'.
-        rewrite in_app_iff; ss; eauto.
-    + ss; clarify; eauto.
-    + exploit (IHCin2 Cout seenx (M :: seenM)).
-      split; eauto.
-      ii. exploit (INV0 M0); eauto.
-      red; ii; ss; eauto.
-      ii; repeat des_hyp; clarify.
-      rewrite eqb_ID_eq in *; ss; clarify. contradict.
-      rw. eauto. rw. eauto.
-      ii. des.
-      exploit x4; eauto. ii; des; clarify; eauto.
-      right. exists e'. rewrite in_app_iff; ss; eauto.
-Qed.
-
-Lemma reach_C_no_t `{Eq T} :
-  forall Cin Cout seenx seenM t,
-  InL (Ptr t) (reach_C seenx seenM Cout Cin) = false.
-Proof.
-  induction Cin; ii; ss; repeat des_goal; repeat des_hyp; clarify.
-  match goal with
-  | |- InL ?a ?b = _ =>
-    destruct (InL a b) eqn:CASE; try reflexivity
-  end.
-  rewrite InL_app_iff in CASE; ss; des.
-  rewrite IHCin1 in *. clarify.
-  rewrite IHCin2 in *. clarify.
-Qed.
-
-Definition reach_C_spec `{Eq T} C res :=
-  (forall e (INe : In e res),
-    valid_edge [] e) /\
-  (forall e (LEFT : Ctx C = lvertex e)
-    (VAL : valid_edge [] e),
-    In e res) /\
-  (forall e e' C (INe : In e res)
-    (INC : Ctx C = lvertex e \/ Ctx C = rvertex e)
-    (LEFT : Ctx C = lvertex e')
-    (VAL : valid_edge [] e'),
-    In e' res) /\
-  (forall e t (LEFT : Ptr t = lvertex e),
-    ~ In e res).
-
-Lemma reach_C_spec_true `{Eq T} :
-  forall C, reach_C_spec C (reach_C [] [] C C).
-Proof.
-  intros.
-  pose proof (reach_C_pre_post C C [] []) as HINT.
-  exploit HINT.
-  unfold reach_C_pre. split; ii; repeat des_goal; clarify.
-  clear HINT. intros HINT.
-  unfold reach_C_post in HINT. des.
-  repeat split; eauto.
-  - ii. destruct e; ss; repeat des_hyp; clarify.
-    exploit HINT; eauto. rw. eauto.
-    exploit HINT0; eauto. rw. eauto.
-  - ii; des.
-    exploit HINT3; eauto. ii. des; clarify.
-    destruct e'; ss; repeat des_hyp; clarify.
-    { exploit HINT; eauto. rw. eauto. }
-    { exploit HINT0; eauto. rw. eauto. }
-    exploit HINT1; eauto.
-    exploit HINT1; eauto.
-  - red; ii.
-    pose proof (reach_C_no_t C C [] [] t).
-    match goal with
-    | _ : InL ?a ?b = false |- _ =>
-      let HINT := fresh "HINT" in
-      assert (InL a b <> true) as HINT;
-      first [apply HINT | refl_bool; ii; clarify]
-    end.
-    rewrite InL_In. exists e. eauto.
-Qed.
-
-Lemma reach_C_path_left `{Eq T} :
-  forall Cin Cout seenx seenM e
-    (PRE : reach_C_pre seenx seenM Cout Cin)
-    (IN : In e (reach_C seenx seenM Cout Cin)),
-    reachable (Ctx Cout) [] e.
-Proof.
-  induction Cin; ii; ss;
-  repeat des_hyp; clarify.
-  - rewrite Inb_eq in *.
-    unfold reach_C_pre in PRE.
-    des; ss.
-    eapply IHCin; eauto.
-    split; eauto.
-    ii. exploit (PRE x0); eauto.
-    ii. repeat des_hyp; clarify.
-    rewrite eqb_ID_eq in *; clarify.
-    rw. eauto. rw. eauto.
-  - rewrite Inb_neq in *.
-    unfold reach_C_pre in PRE.
-    des; clarify.
-    specialize (PRE x HDES).
-    repeat des_hyp; clarify.
-    exists (Px x (Ptr t0) Pnil).
-    ss. rw. eauto.
-    rewrite eqb_ID_neq in *. contradict.
-    rewrite eqb_ID_neq in *. contradict.
-    eapply IHCin; eauto.
-    split; eauto.
-    ii. exploit (PRE x0); eauto.
-    ss. red; ii; eauto.
-    ii. repeat des_hyp; clarify.
-    rewrite eqb_ID_eq in *; clarify; ss; contradict.
-    rw. eauto. rw. eauto.
-  - rewrite Inb_eq in *.
-    unfold reach_C_pre in PRE.
-    des; ss.
-    eapply IHCin2; eauto.
-    split; eauto.
-    ii. exploit (PRE0 M0); eauto.
-    ii. repeat des_hyp; clarify.
-    rewrite eqb_ID_eq in *; clarify.
-    rw. eauto. rw. eauto.
-  - rewrite in_app_iff in *.
-    rewrite Inb_neq in *.
-    ss. des; clarify.
-    + exploit (IHCin1 Cin1 [] [] e); eauto.
-      red; ii. split; ii; repeat des_goal; clarify.
-      ii. unfold reachable in *; des.
-      exists (PM M (Ctx Cin1) p).
-      split; ss; eauto.
-      unfold reach_C_pre in PRE. des.
-      exploit (PRE0 M); eauto.
-      ii. repeat des_hyp; clarify;
-      rewrite eqb_ID_neq in *; contradict.
-    + exists (PM M (Ctx Cin1) Pnil).
-      split; ss; eauto.
-      unfold reach_C_pre in PRE. des.
-      exploit (PRE0 M); eauto.
-      ii. repeat des_hyp; clarify;
-      rewrite eqb_ID_neq in *; clarify.
-    + eapply IHCin2; eauto.
-      unfold reach_C_pre in *; ss; des.
-      split; eauto.
-      ii. exploit (PRE0 M0).
-      red; ii; eauto.
-      ii. repeat des_hyp; clarify.
-      rewrite eqb_ID_eq in *; clarify. contradict.
-      rw. eauto. rw. eauto.
-Qed.
-
-Lemma reach_C_eq_def `{Eq T} :
-  forall C e,
-  reachable (Ctx C) [] e <->
-  In e (reach_C [] [] C C).
-Proof.
-  ii. split; intros REACH.
-  pose proof (reach_C_spec_true C) as SPEC.
-  unfold reach_C_spec in SPEC. des.
-  unfold reachable in *. des.
-  remember (reach_C [] [] C C) as l.
-  clear Heql.
-  ginduction p; ii; ss;
-  repeat des_hyp; clarify; des; clarify.
-  - eapply SPEC0; ss; try rw; eauto.
-  - destruct p; ss; des; clarify;
-    repeat des_hyp; des; clarify.
-  - eapply SPEC0; ss; try rw; eauto.
-  - eapply IHp; eauto. ii.
-    exploit (SPEC1 (EM (Ctx C) M (Ctx d))); ss; eauto.
-    eapply SPEC0; ss; try rw; eauto.
-  - eapply reach_C_path_left; eauto.
-    split; ii; repeat des_goal; eauto.
-Qed.
-
-Lemma no_t_memify_empty `{Eq T} :
-  forall l (NO : forall t, InL (Ptr t) l = false),
-    memify l = [].
-Proof.
-  induction l; ii; ss; repeat des_goal; repeat des_hyp;
-  ss; clarify; eauto;
-  match goal with
-  | NO : forall t, eqb t ?t' || _ = false |- _ =>
-    solve [specialize (NO t'); rewrite t_refl in NO; ss]
-  end.
-Qed.
-
-Lemma reach_C_memify_empty `{Eq T} :
-  forall seenx seenM Cout Cin,
-    memify (reach_C seenx seenM Cout Cin) = [].
-Proof.
-  intros. apply no_t_memify_empty.
-  apply reach_C_no_t.
-Qed.
-
-Definition step_pre `{Eq T}
-  (n : node T) (m : memory T) (E : list (edge T)) :=
-  (forall e,
-    In e E <-> 
-    (valid_edge (memify E) e /\
-      (n = lvertex e \/
-      exists e',
-        In e' E /\
-        rvertex e' = lvertex e))) /\
-  (forall t (IN : InL (Ptr t) E = true),
-    None = read m t).
-
-Lemma reach_C_step_pre `{Eq T} :
-  forall C m, step_pre (Ctx C) m (reach_C [] [] C C).
-Proof.
-  intros. unfold step_pre. split.
-  - intros.
-    rewrite reach_C_memify_empty.
-    rewrite <- reach_C_eq_def.
-    split; ii.
-    rewrite reachable_eq_def in *; des; eauto.
-    rewrite reach_C_eq_def in *. eauto.
-    rewrite reachable_eq_def in *; des; eauto.
-    rewrite <- reach_C_eq_def in *. eauto.
-  - ii. rewrite reach_C_no_t in *. clarify.
-Qed.
-
-Lemma read_memify_In `{Eq T} :
-  forall E (PRE : forall e, In e E -> valid_edge (memify E) e)
-    t x e C,
-    Some (Closure x e C) = read (memify E) t <->
-    In (Ev (Ptr t) (v_fn x e) (Ctx C)) E.
-Proof.
-  ii. split; intros IN.
-  - clear PRE.
-    induction E; ii; ss;
-    repeat des_goal; repeat des_hyp; clarify; 
-    ss; clarify; eauto.
-    rewrite eqb_eq in *; clarify. eauto.
-  - assert (forall x' e' C', 
-      In (Ev (Ptr t) (v_fn x' e') (Ctx C')) E ->
-      x' = x /\ e' = e /\ C' = C).
-    intros x' e' C' IN'.
-    apply PRE in IN, IN'. ss.
-    des. repeat des_hyp; des; clarify.
-    rewrite <- IN in *. clarify.
-    clear PRE.
-    ginduction E; ii; ss;
-    repeat des_goal; repeat des_hyp; clarify;
-    des; clarify; try solve [apply IHE; eauto].
-    rewrite eqb_eq in *. clarify.
-    exploit (H0 x0 e0 C0); eauto. ii; des; clarify.
-    rewrite t_refl in *. clarify.
-Qed.
-
-Lemma step_pre_post_true `{Eq T} :
-  forall n m acc (INV : step_pre n m acc),
-  let (acc', m') := reach_m_step acc m in
-  step_pre n m' acc' /\
-  same (memify acc ++ m) (memify acc' ++ m') /\
-  (exists acc'',
-    acc' = acc'' ++ acc /\
-    (forall t
-      (RIGHT : InR (Ptr t) acc = true)
-      (READ : None <> read m t),
-      exists t',
-        InL (Ptr t') acc'' = true /\
-        None <> read m t') /\
-    (forall t
-      (RIGHT : InR (Ptr t) acc = false),
-      InL (Ptr t) acc'' = false)).
-Proof.
-  induction m; ii;
-  repeat des_goal; repeat des_hyp; ss; clarify.
-  split; eauto.
-  split; ii; eauto.
-  exists []. split. reflexivity.
-  split. ii. contradict. ii; ss.
-  unfold step_pre in INV. des.
-  assert (step_pre n m acc) as PRE.
+  intros ISO.
+  ii. unfold trans_iso_m_pre in ISO. des.
+  assert (reachable (Ctx C2) m2 t') as REACH.
+  { rewrite <- ISO0 in *. assumption. }
+  unfold aIso in *.
+  des_goal; eauto.
+  des.
+  assert (areachable (Ctx (trans_C α' C2)) (trans_m α' (m2 ++ m)) (α' t')).
   {
-    split; eauto. ii.
-    exploit INV0; eauto; ii; ss; repeat des_hyp; clarify.
+    destruct REACH as [p [VALp INp]].
+    apply vpath_less_then_vpath_more with (b := m) in VALp.
+    apply vp_then_avp with (α := α') in VALp.
+    exists (pmap α' p). split; eauto.
+    clear IN GDES VALp.
+    generalize dependent t'.
+    induction p; ii; ss; des; clarify; eauto.
   }
-  repeat des_hyp; ss; clarify. (* 2 goals *)
-  - assert (None = read (memify acc) t) as NREAD.
-    {
-      clear IHm INV HDES PRE.
-      assert (InL (Ptr t) acc = false).
-      refl_bool. intros contra.
-      apply INV0 in contra. rewrite t_refl in *. clarify.
-      clear INV0 n m x e0 C.
-      ginduction acc; ii; ss;
-      repeat des_goal; repeat des_hyp; des; clarify; eauto.
-      ss. clarify.
-      rewrite eqb_eq in *. clarify.
-      rewrite eqb_neq in *. contradict.
-    }
-    split. split; ii. (* 3 goals *)
-    + rewrite in_app_iff. rewrite app_memify.
-      rewrite reach_C_memify_empty. simpl.
-      split; intros IN; des. (* 5 goals *)
-      * rewrite <- reach_C_eq_def in IN.
-        rewrite reachable_eq_def in IN. des; clarify.
-        split. destruct e; repeat des_hyp; ss; clarify.
-        right. exists (Ev (Ptr t) (v_fn x e0) (Ctx C)).
-        rewrite in_app_iff. ss. eauto.
-        split.
-        destruct e; ss; repeat des_hyp; des; clarify.
-        right. exists e'. rewrite in_app_iff. split; eauto.
-        left. rewrite <- reach_C_eq_def. eauto.
-      * clarify. ss. rewrite t_refl.
-        split. exists (Closure x e0 C). eauto.
-        right. rewrite InR_In in HDES. des.
-        exists e. rewrite in_app_iff. ss. eauto.
-      * rewrite INV in IN. destruct IN as [VAL LEFT].
-        split.
-        destruct e; ss; repeat des_hyp; clarify.
-        des; repeat des_hyp; des; clarify;
-        exists (Closure x0 e C0); des_goal; eauto;
-        rewrite eqb_eq in *; clarify; rewrite <- VAL in *; clarify.
-        des; eauto. right. exists e'. rewrite in_app_iff; ss; eauto.
-      * destruct e; ss; repeat des_hyp; des; clarify;
-        match goal with
-        | _ => solve [rewrite eqb_eq in *; des; clarify; eauto]
-        | _ => right; right; rewrite INV; ss; split; eauto
-        end.
-        rw. eauto. rw. eauto.
-      * rewrite in_app_iff in *. ss; des.
-        (* case 1 *)
-        rewrite <- reach_C_eq_def in *.
-        destruct e; ss; repeat des_hyp; clarify;
-        match goal with
-        | |- context [reachable _ _ ?e] =>
-          left; eapply paste_vpath; eauto; rw;
-          match e with
-          | Ex _ ?x ?n =>
-            exists (Px x n Pnil); ss; rw; eauto
-          | EM _ ?M ?n =>
-            exists (PM M n Pnil); ss; rw; eauto
-          end
-        | _ => rewrite eqb_eq in *; repeat (des; clarify; eauto)
-        | _ => right; right; des; des_hyp; des; clarify
-        end.
-        rewrite <- read_memify_In; eauto.
-        ii. rewrite INV in *. des; eauto.
-        (* case 2 *)
-        clarify; ss. left.
-        rewrite <- reach_C_eq_def.
-        rewrite valid_edge_C in IN; eauto.
-        rewrite reachable_eq_def. eauto.
-        (* case 3 *)
-        destruct e; ss; repeat des_hyp; des; clarify;
-        match goal with
-        | _ => solve [rewrite eqb_eq in *; des; clarify; eauto]
-        | _ => right; right; rewrite INV; ss; split; eauto
-        end.
-        rw. eauto. rw. eauto.
-    + rewrite InL_app_iff in *.
-      des. rewrite reach_C_no_t in *. clarify.
-      ss. des_hyp. rewrite eqb_eq in *; clarify.
-      apply remove_t_read.
-      exploit INV0; eauto. des_goal. clarify.
-      rewrite eqb_neq in *.
-      ii. rewrite remove_t_read_some; eauto.
-    + split.
-      * rewrite app_memify. rewrite reach_C_memify_empty. simpl.
-        repeat match goal with
-        | |- context [(?t, ?v) :: ?l] =>
-          lazymatch l with
-          | [] => fail
-          | _ => replace ((t, v) :: l) with ([(t, v)] ++ l) by reflexivity
-          end
-        end.
-        repeat rewrite app_assoc.
-        eapply same_trans.
-        instantiate (1 := (memify acc ++ [(t, Closure x e0 C)]) ++ remove_t m t).
-        repeat rewrite <- app_assoc. apply app_same. ii; ss.
-        ii; ss. des_goal; clarify. rewrite eqb_neq in *.
-        rewrite remove_t_read_some; eauto.
-        apply app_same. apply app_disj_same.
-        ii. ss. des_goal; clarify. rewrite eqb_eq in *. clarify.
-        ii. ss.
-      * exists (reach_C [] [] C C ++ [Ev (Ptr t) (v_fn x e0) (Ctx C)]).
-        split. rewrite <- app_assoc. ss.
-        split. ii. exists t. rewrite t_refl.
-        split; ii; clarify.
-        rewrite InL_In. exists (Ev (Ptr t) (v_fn x e0) (Ctx C)).
-        rewrite in_app_iff. split; ss; eauto.
-        ii. refl_bool. ii.
-        rewrite InL_app_iff in *. des.
-        rewrite reach_C_no_t in *. clarify.
-        ss. des_hyp. rewrite eqb_eq in *. clarify.
-  - exploit IHm; eauto. intros POST.
-    repeat des_hyp; des; clarify.
-    unfold step_pre in POST. des.
-    assert (InL (Ptr t) acc = false) as NIN.
-    refl_bool. ii. exploit INV0; eauto. rewrite t_refl. clarify.
-    assert (InL (Ptr t) acc'' = false) as NIN'. eauto.
-    split; split; try assumption. (* 3 goals *)
-    + ii. exploit POST1; eauto. ii.
-      ss. des_goal; clarify. rewrite eqb_eq in *; clarify.
-      rewrite InL_app_iff in IN. des; clarify.
-    + repeat match goal with
-      | |- context [(?t, ?v) :: ?l] =>
-        lazymatch l with
-        | [] => fail
-        | _ => replace ((t, v) :: l) with ([(t, v)] ++ l) by reflexivity
-        end
-      end.
-      repeat rewrite app_assoc.
-      eapply same_trans.
-      instantiate (1 := ([(t, e)] ++ memify acc) ++ m).
-      apply app_same.
-      apply app_disj_same.
-      ii; ss. des_goal; eauto.
-      rewrite eqb_eq in *. clarify.
-      destruct (read (memify acc) t0) eqn:READ'; clarify.
-      symmetry in READ'.
-      destruct e0. rewrite read_memify_In in *.
-      assert (InL (Ptr t0) acc = true).
-      rewrite InL_In. exists (Ev (Ptr t0) (v_fn x e0) (Ctx C)). ss.
-      clarify.
-      ii. rewrite INV in *. des; eauto.
-      ii; ss.
-      eapply same_trans.
-      instantiate (1 := ([(t, e)] ++ memify (acc'' ++ acc)) ++ l2).
-      repeat rewrite <- app_assoc. ss.
-      solve [ii; ss; des_goal; eauto].
-      apply app_same.
-      apply app_disj_same.
-      ii; ss. des_hyp; clarify.
-      rewrite eqb_eq in *. clarify.
-      match goal with |- None = ?x => destruct x eqn:CASE end; try reflexivity.
-      symmetry in CASE.
-      destruct e0. rewrite read_memify_In in CASE.
-      rewrite in_app_iff in *. des.
-      assert (InL (Ptr t0) acc'' = true).
-      rewrite InL_In. eauto. clarify.
-      assert (InL (Ptr t0) acc = true).
-      rewrite InL_In. eauto. clarify.
-      ii. rewrite POST in *. des; eauto.
-      ii; ss.
-    + exists acc''. split; eauto.
-      split; ii; eauto.
-      des_hyp; clarify.
-      rewrite eqb_eq in *; clarify.
-      exploit POST2; eauto. ii. des.
-      exists t'. des_goal; clarify.
-Qed.
-
-Lemma step_spec_left `{Eq T} :
-  forall E n
-    (PRE : forall e, (valid_edge (memify E) e /\
-      (n = lvertex e \/
-      exists e',
-        In e' E /\
-        rvertex e' = lvertex e)) -> In e E)
-    e (REACH : reachable n (memify E) e),
-  In e E.
-Proof.
-  ii.
-  unfold reachable in REACH. des.
-  ginduction p; ii; ss; repeat des_hyp; clarify;
-  des; clarify; try des_hyp; des; clarify.
-  - apply PRE. ss. rw. eauto.
-  - eapply IHp with (n := (Ptr t0)); eauto.
-    ii. apply PRE. split; des; eauto.
-    right. exists (Ex (Ctx C) x (Ptr t0)).
-    split; ss; eauto. apply PRE. ss. rw. eauto.
-  - apply PRE. ss. rw. eauto.
-  - eapply IHp with (n := (Ctx d)); eauto.
-    ii. apply PRE. split; des; eauto.
-    right. exists (EM (Ctx C0) M (Ctx d)).
-    split; ss; eauto. apply PRE. ss. rw. eauto.
-  - apply PRE. ss. split; eauto.
-    exists (Closure x e C0); ss.
-  - eapply IHp with (n := (Ctx C0)); eauto.
-    ii. apply PRE. split; des; eauto.
-    right. exists (Ev (Ptr t) (v_fn x e0) (Ctx C0)).
-    split; ss; eauto. apply PRE. ss. split; eauto.
-    exists (Closure x e0 C0); ss.
-Qed.
-
-Lemma vpath_less_then_vpath_more `{Eq T} :
-  forall a b p n (VAL : valid_path n a p),
-  valid_path n (a ++ b) p.
-Proof.
-  ii.
-  ginduction p; ii; ss;
-  repeat des_hyp; des; clarify; eauto.
-  des_hyp; des; clarify.
-  exists (Closure x e C0).
-  rewrite read_top. rewrite <- VAL. eauto.
-Qed.
-
-Lemma vedge_less_then_vedge_more `{Eq T} :
-  forall a b e (VAL : valid_edge a e),
-  valid_edge (a ++ b) e.
-Proof.
-  ii.
-  destruct e; ss; repeat des_hyp; des; clarify.
-  des_hyp; des; clarify.
-  exists (Closure x e C).
-  rewrite read_top. rewrite <- VAL. eauto.
-Qed.
-
-Lemma step_spec_right `{Eq T} :
-  forall m n E
-    (PRE : forall e, In e E -> reachable n (memify E) e)
-    (DISJ : forall t, InL (Ptr t) E = true -> None = read m t),
-    let (E', m') := reach_m_step E m in
-    (forall e (IN : In e E'), reachable n (memify E') e) /\
-    (forall t (LEFT : InL (Ptr t) E' = true), None = read m' t) /\
-    (forall t (LEFT : InL (Ptr t) E' = true /\ InL (Ptr t) E = false),
-      InR (Ptr t) E = true).
-Proof.
-  ii.
-  match goal with
-  | |- match ?E with _ => _ end =>
-    destruct E as [E' m'] eqn:STEP
-  end; ii.
-  ginduction m; ii; ss; clarify; eauto.
-  assert (forall e, In e E' -> valid_edge (memify E') e) as HINT.
+  exploit (ISO9 _ (trans_v α' e)); eauto.
   {
-    ii. exploit PRE; eauto. ii.
-    rewrite reachable_eq_def in *. des; eauto.
+    rewrite trans_m_aread.
+    rewrite <- disj_reflect in ISO.
+    exploit (ISO t'). rw. ii; clarify. ii.
+    exists t'. exists e. rewrite read_top. rrw. eauto.
   }
-  repeat split; eauto. ii.
-  {
-    des. rewrite InL_In in LEFT. des.
-    apply PRE in LEFT. rewrite reachable_eq_def in LEFT.
-    destruct LEFT as [VAL ?].
-    destruct e; ss; repeat des_hyp; des; clarify;
-    des_hyp; des; clarify;
-    rewrite read_memify_In in VAL; eauto;
-    assert (InL (Ptr t0) E' = true);
-    solve [rewrite InL_In; exists (Ev (Ptr t0) (v_fn x e) (Ctx C)); eauto | clarify].
-  }
-  des_hyp.
-  assert (InL (Ptr t) E = false) as DISJ'.
-  { refl_bool. intros contra. apply DISJ in contra. rewrite t_refl in *. clarify. }
-  assert (forall e, In e E -> valid_edge (memify E) e) as HINT.
-  {
-    ii. exploit PRE; eauto. ii.
-    rewrite reachable_eq_def in *. des; eauto.
-  }
-  split.
-  repeat des_hyp; clarify; ii.
-  - rewrite InR_In in *. des. rename IN into IN'.
-    match goal with
-    | H : _ |- _ => 
-      apply PRE in H;
-      unfold reachable in H;
-      destruct H as [p [VAL IN]]
-    end.
-    rewrite app_memify. rewrite reach_C_memify_empty. s.
-    assert (forall p', valid_path n (memify E) p' -> 
-      valid_path n ((t, Closure x e0 C) :: memify E) p').
-    {
-      clear IHm PRE DISJ e1 IN HDES1 e IN'.
-      ii. ginduction p'; ii; ss;
-      repeat des_goal; des; clarify; eauto.
-      rewrite eqb_eq in *. clarify.
-      des. des_hyp. rewrite read_memify_In in *; eauto.
-      des; clarify.
-      assert (InL (Ptr t0) E = true).
-      rewrite InL_In. eauto. clarify.
-      des. des_hyp. des. clarify.
-      exists (Closure x0 e C1); eauto.
-    }
-    rewrite in_app_iff in *.
-    ss. des; clarify.
-    + rewrite <- reach_C_eq_def in IN'.
-      eapply paste_vpath. instantiate (1 := e1).
-      exists p. split; eauto.
-      rrw.
-      match goal with
-      | _ : context [(?t, Closure ?x ?e ?C)] |- _ =>
-        eapply paste_vpath;
-        first [
-          instantiate (1 := (Ev (Ptr t) (v_fn x e) (Ctx C)));
-          exists (Pv (v_fn x e) (Ctx C) Pnil);
-          ss; rewrite t_refl; split; eauto;
-          exists (Closure x e C); eauto |
-          idtac]
-      end.
-      ss. destruct IN' as [p' [VAL' IN']].
-      exists p'. split; eauto.
-      eapply vpath_less_then_vpath_more with (a := []). eauto.
-    + eapply paste_vpath. instantiate (1 := e1). exists p. split; eauto.
-      rrw.
-      match goal with
-      | _ : context [(?t, Closure ?x ?e ?C)] |- _ =>
-        exists (Pv (v_fn x e) (Ctx C) Pnil);
-        ss; rewrite t_refl; split; eauto;
-        exists (Closure x e C); eauto
-      end.
-    + apply PRE in IN'.
-      destruct IN' as [p' [VAL' IN']].
-      exists p'. eauto.
-  - exploit IHm; ii; des; eauto.
-    exploit DISJ; eauto.
-    des_goal; clarify.
-  - repeat des_hyp; clarify. repeat split.
-    + ii. rewrite InL_app_iff in LEFT.
-      des. rewrite reach_C_no_t in LEFT. clarify.
-      ss. des_hyp. rewrite eqb_eq in *; clarify.
-      apply remove_t_read.
-      exploit DISJ; eauto.
-      ii. des_hyp; clarify.
-      rewrite eqb_neq in *.
-      rewrite remove_t_read_some; eauto.
-    + ii. rewrite InL_app_iff in LEFT.
-      des. rewrite reach_C_no_t in LEFT. clarify.
-      ss. des_hyp; clarify. rewrite eqb_eq in *; clarify.
-    + exploit IHm; ii; des; eauto.
-      exploit DISJ; eauto.
-      des_goal; clarify.
-      repeat split; eauto.
-      ii. ss. des_goal; eauto.
-      rewrite eqb_eq in *. clarify.
-      assert (InR (Ptr t0) E = true).
-      eauto. clarify.
+  ii; des. exists v'. split; eauto.
+  repeat des_hyp; des; clarify.
+  rewrite <- check_aiso_aiso in *.
+  rewrite <- iso_C_is_aiso_C in *.
+  rewrite check_iso_iso in *. eauto.
 Qed.
 
-Lemma step_spec_lemma `{Eq T} :
-  forall m n E
-    (IN : forall e, In e E <-> reachable n (memify E) e)
-    (DISJ : forall t, InL (Ptr t) E || InR (Ptr t) E = true ->
-      None = read m t)
-    (INn : InL n E || InR n E = true) e,
-    In e E <-> reachable n (memify E ++ m) e.
+Lemma pmap_fst_read `{Eq T} `{Eq TT} (ϕ: list (T * TT)) :
+  forall p p' t (MAP : pmap_fst ϕ p = Some p') (IN : Inp t p),
+  None <> read_fst ϕ t.
 Proof.
-  ii. rewrite IN.
-  split; intros REACH;
-  destruct REACH as [p [VAL INV]];
-  exists p; split; try assumption.
-  apply vpath_less_then_vpath_more. eauto.
-  assert (forall e, reachable n (memify E) e -> In e E) as REACH.
-  ii. rewrite IN. eauto.
-  clear IN e INV.
-  ginduction p; ii; ss;
-  repeat des_goal; des; clarify.
-  - exploit (REACH (Ex (Ctx C) x (Ptr t0))).
-    exists (Px x (Ptr t0) Pnil). ss. rw. eauto.
-    ii.
-    assert (InR (Ptr t0) E = true).
-    rewrite InR_In. eauto.
-    split; eauto. eapply IHp; eauto. rw. des_goal; eauto.
-    intros e' REACH'. apply REACH.
-    eapply paste_vpath.
-    instantiate (1 := Ex (Ctx C) x (Ptr t0)).
-    exists (Px x (Ptr t0) Pnil). ss. rw. eauto.
-    ss.
-  - exploit (REACH (EM (Ctx C0) M (Ctx d))).
-    exists (PM M (Ctx d) Pnil). ss. rw. eauto.
-    ii.
-    assert (InR (Ctx d) E = true).
-    rewrite InR_In. exists (EM (Ctx C0) M (Ctx d)). ss.
-    split; eauto. eapply IHp; eauto. rw. des_goal; eauto.
-    intros e' REACH'. apply REACH.
-    eapply paste_vpath.
-    instantiate (1 := EM (Ctx C0) M (Ctx d)).
-    exists (PM M (Ctx d) Pnil). ss. rw. eauto.
-    ss.
-  - destruct ev; des; clarify.
-    rewrite read_top in *.
-    destruct (read (memify E) t) eqn:READ.
-    + clarify. exists (Closure x e C0).
-      repeat split; eauto.
-      eapply IHp; eauto.
-      assert (InR (Ctx C0) E = true).
-      rewrite InR_In.
-      exists (Ev (Ptr t) (v_fn x e) (Ctx C0)).
-      split; eauto. apply REACH.
-      exists (Pv (v_fn x e) (Ctx C0) Pnil).
-      ss. split; eauto. exists (Closure x e C0); eauto.
-      rw. des_goal; eauto.
-      intros e' REACH'. apply REACH.
-      eapply paste_vpath.
-      instantiate (1 := Ev (Ptr t) (v_fn x e) (Ctx C0)).
-      exists (Pv (v_fn x e) (Ctx C0) Pnil).
-      ss. split; eauto. exists (Closure x e C0); eauto.
-      ss.
-    + assert (None = read m t) as RR.
-      apply DISJ. rw. eauto.
-      rewrite <- RR in *. clarify.
+  induction p; ii; ss; repeat des_hyp; des; clarify.
+  all:try solve [exploit IHp; eauto].
+  rewrite HDES in *. clarify.
 Qed.
 
-Lemma iso_comm `{Eq T} `{Eq TT} :
-  forall (C : dy_ctx T) m (C' :dy_ctx TT) m' f f',
-  iso C m C' m' f f' <-> iso C' m' C m f' f.
+Lemma pmap_snd_read `{Eq T} `{Eq TT} (ϕ: list (T * TT)) :
+  forall p p' t (MAP : pmap_snd ϕ p = Some p') (IN : Inp t p),
+  None <> read_snd ϕ t.
 Proof.
-  ii; split; ii; unfold iso in *; des;
-  repeat (split; eauto).
-Qed.
-
-Lemma asame_comm `{Eq T} :
-  forall m m',
-  asame m m' <-> asame m' m.
-Proof.
-  intros; unfold asame; split; ii; rw; eauto.
-Qed.
-
-Lemma aiso_comm `{Eq T} `{Eq TT} :
-  forall (C : dy_ctx T) m (C' :dy_ctx TT) m' f f',
-  aiso C m C' m' f f' <-> aiso C' m' C m f' f.
-Proof.
-  ii; split; ii; unfold aiso in *; des;
-  repeat (split; eauto).
-Qed.
-
-Lemma same_valid `{Eq T} :
-  forall p n m m' (SAME : same m m')
-    (VALp : valid_path n m p),
-  valid_path n m' p.
-Proof.
-  ii; unfold same in *;
-  ginduction p; intros; ss;
-  repeat des_goal; repeat des_hyp; clarify;
-  des; try split; eauto.
-  - exists ev. split. rewrite <- SAME. eauto.
-    des_hyp; des; clarify; eauto.
+  induction p; ii; ss; repeat des_hyp; des; clarify.
+  all:try solve [exploit IHp; eauto].
+  rewrite HDES in *. clarify.
 Qed.
 
 Lemma asame_avalid `{Eq T} :
-  forall p n m m' (SAME : asame m m')
-    (VALp : avalid_path n m p),
-  avalid_path n m' p.
+  forall p r m1 m2 (SAME : asame m1 m2),
+    avalid_path r m1 p <-> avalid_path r m2 p.
 Proof.
-  ii; unfold asame in *;
-  ginduction p; intros; ss;
-  repeat des_goal; repeat des_hyp; clarify;
-  des; try split; eauto.
-  - exists ev. split. rewrite <- SAME. eauto.
-    des_hyp; des; clarify; eauto.
+  induction p; ii; ss; split; ii; repeat des_hyp; des; clarify.
+  rw; eauto. unfold asame in *. ii. rw. eauto.
+  rw; eauto. rw; eauto. unfold asame in *; ii; rw; eauto.
+  rw; eauto.
+  des_hyp; des; clarify. unfold asame in SAME. rewrite SAME in *.
+  eexists. split; eauto. s. rw; eauto. ii. rw. eauto.
+  des_hyp; des; clarify. unfold asame in SAME. rewrite <- SAME in *.
+  eexists. split; eauto. s. rw; eauto.
 Qed.
 
-Lemma same_equiv `{Eq T} `{Eq TT} :
-  forall (V : dy_value T) m (V' : dy_value TT) m' m''
-    (EQUIV : <|V m ≃ V' m'|>) (SAME : same m' m''),
-  <|V m ≃ V' m''|>.
+Lemma asame_aIso `{Eq T} `{Eq TT} (φ : T -> TT) φ' :
+  forall r m1 m2 r' m' (SAME : asame m1 m2) (ISO : aIso r m2 r' m' φ φ'),
+  aIso r m1 r' m' φ φ'.
 Proof.
-  intros. red in EQUIV; repeat des_hyp; des; clarify; red;
-  repeat split; try reflexivity; exists f; exists f';
-  unfold iso in *; des;
-  (split; 
-  first [assumption | split];
-  first [assumption | split]); ii;
-  match goal with
-  | H : _ |- context [valid_path (Ctx ?C) m''] =>
-    specialize (H p VALp); des; split; eauto;
-    remember (pmap f p) as p';
-    remember (Ctx C) as n;
-    clear Heqn Heqp' VALp
-  | H : context [valid_path (Ctx ?C) m'] |- _ =>
-    apply H; remember (Ctx C) as n;
-    clear Heqn
-  end; 
-  solve [eapply same_valid; eauto |
-  rewrite same_comm in *; eapply same_valid; eauto].
+  ii. destruct ISO as [[ISO ISO'] [ISO'' ISO''']]. ss.
+  split. split; ss.
+  ii. apply ISO. rewrite asame_avalid in *; eauto.
+  split; ii; ss.
+  ii. rewrite asame_avalid; eauto.
+  split; ii. destruct REACH as [p [VALp INp]].
+  apply ISO''. exists p. split; eauto. rewrite <- asame_avalid; eauto.
+  unfold asame in SAME. rewrite <- SAME. eauto.
+  exploit ISO'''; eauto. ii; des.
+  exists v.
+  unfold asame in *. rewrite SAME. eauto.
 Qed.
 
-
-Lemma asame_aequiv `{Eq T} `{Eq TT} :
-  forall (V : dy_value T) m (V' : dy_value TT) m' m''
-    (EQUIV : <|V m ≃# V' m'|>) (SAME : asame m' m''),
-  <|V m ≃# V' m''|>.
+Lemma trans_m_iso_pre_post `{Eq TT} `{Eq aTT} `{TotalOrder T} `{Eq aT}
+  n (α' : TT -> aTT) (inv_α : (T * aT) -> T) (α : T -> aT) φ φ'
+  (ϕ : list (TT * T)) (tϕ : T) (C2 : dy_ctx TT) (C1 : dy_ctx T)
+  (am : memory aT) (m1 : memory T) (m2 m : memory TT)
+  (LE : length m <= n)
+  (PRE : trans_iso_m_pre α' inv_α α φ φ' ϕ tϕ C2 C1 am m1 m2 m) :
+  match trans_iso_m_aux α' inv_α φ φ' ϕ tϕ am m1 m2 m n with
+  | Fix _ _ _ _ _ => True
+  | Unfix => False
+  end.
 Proof.
-  intros. red in EQUIV; repeat des_hyp; des; clarify; red;
-  repeat split; try reflexivity; exists f; exists f';
-  unfold aiso in *; des;
-  (split; 
-  first [assumption | split];
-  first [assumption | split]); ii;
-  match goal with
-  | H : _ |- context [avalid_path (Ctx ?C) m''] =>
-    specialize (H p VALp); des; split; eauto;
-    remember (pmap f p) as p';
-    remember (Ctx C) as n;
-    clear Heqn Heqp' VALp
-  | H : context [avalid_path (Ctx ?C) m'] |- _ =>
-    apply H; remember (Ctx C) as n;
-    clear Heqn
-  end;
-  solve [eapply asame_avalid; eauto |
-  rewrite asame_comm in *; eapply asame_avalid; eauto].
+  ginduction n; ii; ss.
+  destruct m; ss; nia.
+  apply pre_implies_pre in PRE as PRE'.
+  unfold trans_iso_m_pre in PRE. des.
+  exploit (@trans_m_step_pre_post TT _ aTT _ T _ _ aT); eauto.
+  intros POST. unfold trans_m_step_post in *.
+  repeat des_hyp; eauto.
+  des; clarify.
+  assert (trans_iso_m_pre α' inv_α α φ φ' (ϕ' ++ ϕ) tϕ0 C2 C1 am
+    ((t', Closure x0 e0 C0) :: m1) ((t, Closure x0 e0 C) :: m2)
+    (remove_t m t)).
+  {
+    split; ii; ss. des_hyp. rewrite eqb_eq in *; clarify.
+    erewrite remove_t_read; eauto.
+    exploit PRE; eauto. erewrite remove_t_read_some; eauto.
+    rewrite <- eqb_neq. eauto.
+    assert (read m2 t = None) as DISJ.
+    destruct (read m2 t) eqn:CASE; eauto.
+    exploit (PRE t). rw. ii; clarify.
+    repeat rrw. ii; clarify.
+    (* reachable <-> read_fst *)
+    split; ii.
+    split; intros REACH. apply tail_vpath in REACH.
+    des; clarify.
+    destruct REACH as [p [VALp INp]].
+    apply vpath_less_then_vpath_more with (b := m2) in VALp; ss.
+    assert (None <> read_fst ϕ t0). rewrite <- PRE0. exists p. eauto.
+    rewrite read_fst_top.
+    repeat des_goal; clarify.
+    destruct (eqb t t'0) eqn:CASE.
+    rewrite eqb_eq in *. clarify. ss. rewrite t_refl in *. clarify.
+    destruct REACH1 as [p [VALp INp]].
+    exploit POST7; eauto.
+    des_goal; clarify.
+    ii. exploit (pmap_fst_read (ϕ' ++ ϕ) p); eauto.
+    ss. rewrite CASE in *. destruct REACH1 as [p [VALp INp]].
+    exploit PRE3; eauto.
+    ii. repeat des_hyp; des; clarify.
+    exploit (pmap_fst_read ϕ p); eauto.
+    rewrite read_fst_top in *. repeat des_hyp; clarify.
+    assert (reachable (Ctx C2) m2 t) as REACH'.
+    { rewrite PRE0. rrw. ii; clarify. }
+    rewrite read_fst_top in *. repeat des_hyp; clarify.
+    exploit (POST8 t0). rw. ii; clarify. intros [p [VALp INp]].
+    apply paste_vpath with (t := t).
+    apply reachable_disj with (m' := [(t, Closure x0 e0 C)]); eauto.
+    rewrite <- disj_reflect. ii; ss.
+    des_hyp; clarify. rewrite eqb_eq in *; clarify.
+    exists (Pv (v_fn x0 e0) p). s. split; eauto.
+    rewrite t_refl. eexists. split; eauto.
+    s. split; eauto.
+    exploit (vpath_less_then_vpath_more [] _ p (Ctx C)); eauto.
+    rewrite <- PRE0 in REACH.
+    apply reachable_disj with (m' := [(t, Closure x0 e0 C)]); eauto.
+    rewrite <- disj_reflect. ii; ss.
+    des_hyp; clarify. rewrite eqb_eq in *; clarify.
+    (* equiv_fst_ϕ_C *)
+    split; ii. exploit PRE1; eauto. ii. des_hyp.
+    erewrite (@pmap_fst_app TT _ aTT _ T _ _ aT); eauto.
+    (* equiv_snd_ϕ_C *)
+    split; ii. exploit PRE2; eauto. ii. des_hyp.
+    erewrite (@pmap_snd_app TT _ aTT _ T _ _ aT); eauto.
+    (* equiv_fst_ϕ_m *)
+    split; ii; ss. des_hyp; clarify.
+    rewrite eqb_eq in *. clarify. exploit POST7; eauto.
+    assert (read_fst (ϕ' ++ ϕ) t0 = Some t').
+    {
+      apply read_fst_in in POST.
+      exploit (POST4 t0 t'). rewrite in_app_iff; eauto.
+      ii. des. rrw. eauto.
+    }
+    rw. ii. des_hyp. rewrite t_refl. eexists. split; eauto.
+    exploit PRE3; eauto.
+    ii. repeat des_hyp; des; clarify.
+    assert (read_fst (ϕ' ++ ϕ) t0 = Some t1).
+    {
+      symmetry in HDES1.
+      apply read_fst_in in HDES1.
+      exploit (POST4 t0 t1). rewrite in_app_iff; eauto.
+      ii. des. rrw. eauto.
+    }
+    rw. erewrite (@pmap_fst_app TT _ aTT _ T _ _ aT); eauto.
+    assert (eqb t' t1 = false).
+    {
+      rewrite eqb_neq. ii. clarify.
+      apply read_fst_in in POST.
+      exploit (PRE5 t t1); eauto. ii; des.
+      symmetry in HDES1. apply read_fst_in in HDES1.
+      exploit (PRE5 t0 t1); eauto. ii; des.
+      rewrite <- x3 in *. clarify. rewrite t_refl in *. clarify.
+    }
+    rw. eexists. split; eauto.
+    (* equiv_snd_ϕ_m *)
+    split; ii; ss. des_hyp; clarify.
+    rewrite eqb_eq in *. clarify. exploit POST6; eauto.
+    assert (read_snd (ϕ' ++ ϕ) t0 = Some t).
+    {
+      apply read_fst_in in POST.
+      exploit (POST4 t t0). rewrite in_app_iff; eauto.
+      ii. des. rrw. eauto.
+    }
+    rw. ii. des_hyp. rewrite t_refl. eexists. split; eauto.
+    exploit PRE4; eauto.
+    ii. repeat des_hyp; des; clarify.
+    assert (read_snd (ϕ' ++ ϕ) t0 = Some t1).
+    {
+      symmetry in HDES1.
+      apply read_snd_in in HDES1.
+      exploit (POST4 t1 t0). rewrite in_app_iff; eauto.
+      ii. des. rrw. eauto.
+    }
+    rw. erewrite (@pmap_snd_app TT _ aTT _ T _ _ aT); eauto.
+    assert (eqb t t1 = false).
+    {
+      rewrite eqb_neq. ii. clarify.
+      apply read_fst_in in POST.
+      exploit (PRE5 t1 t'); eauto. ii; des.
+      symmetry in HDES1. apply read_snd_in in HDES1.
+      exploit (PRE5 t1 t0); eauto. ii; des.
+      rewrite <- x4 in *. clarify. rewrite t_refl in *. clarify.
+    }
+    rw. eexists. split; eauto.
+    (* ϕ_spec *)
+    split; eauto.
+    (* inv_α_spec *)
+    split; eauto.
+    (* aIso *)
+    split.
+    assert (asame (trans_m α' ((t, Closure x0 e0 C) :: m2 ++ remove_t m t)) (trans_m α' (m2 ++ m))).
+    {
+      apply trans_m_asame.
+      apply same_trans with (m' := m2 ++ ([(t, Closure x0 e0 C)] ++ remove_t m t)).
+      rewrite app_assoc.
+      match goal with
+      | |- context [?a :: ?b ++ ?c] =>
+        replace (a :: b ++ c) with (([a] ++ b) ++ c) by reflexivity
+      end.
+      apply app_same.
+      apply app_disj_same. ii; ss. des_hyp; clarify.
+      rewrite eqb_eq in *. clarify.
+      split; ii; ss.
+      apply app_same. split; ii; ss.
+      split; ii; ss.
+      repeat des_hyp; clarify. rewrite eqb_eq in *. clarify.
+      rewrite remove_t_read_some in *; eauto. rewrite eqb_neq in *. eauto.
+      des_goal. rewrite eqb_eq in *. clarify. repeat rw. eauto.
+      rewrite remove_t_read_some; eauto. rewrite eqb_neq in *. eauto.
+    }
+    eapply asame_aIso; eauto.
+    (* In trans_v aread *)
+    ii. des_hyp; eauto.
+    rewrite eqb_eq in *. clarify.
+  }
+  apply IHn with (α := α) (C2 := C2) (C1 := C1); eauto.
+  exploit (remove_t_strict_dec m t).
+  rrw. ii; clarify. nia.
 Qed.
-
-(* lift unreachable Cs *)
-Fixpoint lift_C `{Eq T} `{Eq aT}
-  (inv_α : (T * aT) -> T) (t : T) (C : dy_ctx aT) :=
-  match C with
-  | [||] => [||]
-  | dy_binde x tx C =>
-    let tx := inv_α (t, tx) in
-    let C := lift_C inv_α t C in
-    dy_binde x tx C
-  | dy_bindm M C_M C =>
-    let C_M := lift_C inv_α t C_M in
-    let C := lift_C inv_α t C in
-    dy_bindm M C_M C
-  end.
-
-Fixpoint fst_trans `{Eq T} `{Eq TT} 
-  (trans : list (node T * node TT)) (n : node T) :=
-  match trans with
-  | [] => None
-  | (f, s) :: tl =>
-    if eqb f n then Some s else fst_trans tl n
-  end.
-
-Fixpoint snd_trans `{Eq T} `{Eq TT} 
-  (trans : list (node T * node TT)) (n : node TT) :=
-  match trans with
-  | [] => None
-  | (f, s) :: tl =>
-    if eqb s n then Some f else snd_trans tl n
-  end.
-
-(* for convenience: UNICODE ϕ φ *)
-(* assumed : f (α C) ≃# aC except for paths starting with
- * x in seenx and M in seenM, when f is a graph isomorphism *)
-(* trans: holds translated equivalent nodes *)
-Fixpoint trans_equiv_C_aux `{Eq T} `{Eq TT} `{Eq aTT}
-  (inv_α : (TT * aTT) -> TT)
-  (t : TT) (ϕ : list (node T * node TT)) seenx seenM
-  (C : dy_ctx T) (aC : dy_ctx aTT) :=
-  match fst_trans ϕ (Ctx C) with
-  | Some (Ctx C) => Some (t, ϕ, C) (* already translated *)
-  | Some (Ptr _) => None
-  | None =>
-  let ret := match aC with
-  | [||] => Some (t, ϕ, [||])
-  | dy_binde x tx aC =>
-    if Inb x seenx then (* unreachable *)
-      let tx := inv_α (t, tx) in
-      match trans_equiv_C_aux inv_α t ϕ seenx seenM C aC with
-      | None => None
-      | Some (t, ϕ, C) => Some (t, ϕ, dy_binde x tx C)
-      end
-    else match addr_x C x with (* reachable *)
-    | None => None
-    | Some addr =>
-      let seenx := x :: seenx in
-      match fst_trans ϕ (Ptr addr) with
-      | Some (Ctx _) => None
-      | Some (Ptr tx) =>
-        match trans_equiv_C_aux inv_α t ϕ seenx seenM C aC with
-        | None => None
-        | Some (t, ϕ, C) => Some (t, ϕ, dy_binde x tx C)
-        end
-      | None =>
-        let tx := inv_α (t, tx) in
-        let ϕ := (Ptr addr, Ptr tx) :: ϕ in
-        match trans_equiv_C_aux inv_α tx ϕ seenx seenM C aC with
-        | None => None
-        | Some (t, ϕ, C) => Some (t, ϕ, dy_binde x tx C)
-        end
-      end
-    end
-  | dy_bindm M C_M aC =>
-    if Inb M seenM then (* unreachable *)
-      let C_M := lift_C inv_α t C_M in
-      match trans_equiv_C_aux inv_α t ϕ seenx seenM C aC with
-      | None => None
-      | Some (t, ϕ, C) => Some (t, ϕ, dy_bindm M C_M C)
-      end
-    else match ctx_M C M with (* reachable *)
-    | None => None
-    | Some C_M' =>
-      let seenM := M :: seenM in
-      match trans_equiv_C_aux inv_α t ϕ [] [] C_M' C_M with
-      | None => None
-      | Some (t, ϕ, C_M) =>
-        match trans_equiv_C_aux inv_α t ϕ seenx seenM C aC with
-        | None => None
-        | Some (t, ϕ, C) => Some (t, ϕ, dy_bindm M C_M C)
-        end
-      end
-    end
-  end in
-  let top := match seenx, seenM with
-  | [], [] => true
-  | _, _ => false
-  end in
-  match ret with
-  | None => None
-  | Some (t, ϕ, C') =>
-    if top
-    then Some (t, (Ctx C, Ctx C') :: ϕ, C')
-    else Some (t, ϕ, C')
-  end end.
-
-
-Definition trans_equiv_m :=
-  (* check oracle, if reachable trans_equiv_C
-     if unreachable lift_C *)
-0.
-
-Definition trans_equiv := 0.
-*)
